wip, more refactoring

src/Bedrock/Field/FieldExtensions/QuadraticFieldExtensions.v
@@ -4,6 +4,8 @@ Require Import Crypto.Bedrock.Specs.Field.
 Require Import Crypto.Bedrock.Field.FieldExtensions.Theory.QuadraticExtensions.
 Require Import Crypto.Bedrock.Field.Interface.Compilation2.
 Require Export Crypto.Spec.ModularArithmetic.
+Require Import bedrock2.NotationsCustomEntry.
+Require Import bedrock2.WeakestPrecondition.
 
 (*Move elsewhere*)
 Lemma firstn_skipn {A : Type} : forall (l : list A) n, (firstn n l) ++ (skipn n l) = l.
@@ -71,32 +73,34 @@ Section Fp2.
   Context {prime_parameters : PrimeParameters}
           {prime_parameters_ok : PrimeParameters_ok}
           {M_mod : (Z.pos M_pos) mod 4 =? 3 = true}.
-  Context {F_names : FieldNames}.
-
-  Existing Instance prime_field_parameters.
-  Context {F_representation : FieldRepresentation (F M_pos)}
-          {F_representation_ok : FieldRepresentation_ok (F M_pos)}.
-
-  (* Check _ : FieldParameters. *)
-  (* Instance prime_field_parameters. *)
-  (* Instance F_parameters : FieldParameters := QuadraticFieldExtensionsSpecs.F_parameters. *)
-  (* Instance F_parameters_ok : FieldParameters_ok := QuadraticFieldExtensionsSpecs.F_parameters_ok. *)
-
-  Context {bounds_equiv : forall x, bounded_by loose_bounds x -> bounded_by tight_bounds x}.
 
   Local Notation F := (F M_pos).
   Local Notation Fp2 := ((F * F)%type).
+
+  Existing Instance prime_field_parameters.
+  Context {F_names : FieldNames F}.
+  Context {F_representation : FieldRepresentation F}
+          {F_representation_ok : FieldRepresentation_ok F}.
+
+  Context {bounds_equiv : forall x, bounded_by loose_bounds x -> bounded_by tight_bounds x}.
+
+  Instance spec_of_F_felem_copy : spec_of (felem_copy (F:=F)) := spec_of_felem_copy (F:=F).
+  Instance spec_of_F_select_znz : spec_of (select_znz (F:=F)) := spec_of_selectznz (F:=F).
+  Instance spec_of_F_add : spec_of (add (F:=F)) := binop_spec (bin_add (F:=F)).
+  Instance spec_of_F_mul : spec_of (mul (F:=F)) := binop_spec (bin_mul (F:=F)).
+  Instance spec_of_F_sub : spec_of (sub (F:=F)) := binop_spec (bin_sub (F:=F)).
 
   Local Arguments Field.FElem _ {_ _ _ _ _ _}.
   Local Arguments felem_size_in_words _ {_ _ _ _ _ _}.
   Local Arguments felem_size_in_bytes _ {_ _ _ _ _ _}.
 
-  Instance spec_of_mul : spec_of (@mul _).
-  Proof.
-    pose proof (binop_spec bin_mul). cbv [spec_of]. eapply X.
-  Defined.
+  Local Notation felem_offset := (Memory.bytes_per_word width * Z.of_nat (felem_size_in_words F)).
+  Local Notation felem_offset_word := (word.of_Z felem_offset).
 
-  Definition Fp2_add_F (x y : (ModularArithmetic.F.F M_pos) * (ModularArithmetic.F.F M_pos)) : (ModularArithmetic.F.F M_pos) * (ModularArithmetic.F.F M_pos) := addp2 M_pos x y.
+  Existing Instance Fp2_field_parameters.
+  Existing Instance Fp2_field_parameters_ok.
+  Existing Instance Fp2_field_representation.
+  Existing Instance Fp2_field_representation_ok.
 
   Lemma fst_felem_app : forall a b pa Ra m, (Field.FElem F pa a * Ra)%sep m
     -> fst_felem (a ++ b) = a.
@@ -116,19 +120,6 @@ Section Fp2.
   Proof.
     intros. cbv [fst_felem snd_felem]. rewrite firstn_skipn. auto.
   Qed.
-
-  Local Notation felem_offset := (Memory.bytes_per_word width * Z.of_nat (felem_size_in_words F)).
-  (* Local Notation felem_offset := (felem_size_in_bytes F). *)
-  Local Notation felem_offset_word := (word.of_Z felem_offset).
-
-  Existing Instance Fp2_parameters.
-    (* : FieldParameters := Fp2_parameters. *)
-  Existing Instance Fp2_parameters_ok.
-    (* : FieldParameters_ok := @Fp2_parameters_ok prime_field_parameters prime_field_parameters_ok M_mod. *)
-  Existing Instance Fp2_representation.
-    (* : FieldRepresentation := Fp2_representation. *)
-  Existing Instance Fp2_representation_ok.
-    (* : FieldRepresentation_ok := Fp2_representation_ok. *)
 
   Lemma Fp_FElem_to_Fp2_sep : forall px x m,
     ((Field.FElem F px (fst_felem x)) * (Field.FElem F (word.add px felem_offset_word) (snd_felem x)))%sep m -> (Field.FElem Fp2 px x m).
@@ -209,110 +200,49 @@ Section Fp2.
     apply Fp2_FElem_to_Fp_sep. auto.
   Qed.
 
-  Require Import bedrock2.NotationsCustomEntry.
-  Require Import bedrock2.WeakestPrecondition.
-  Import Syntax BinInt String List.ListNotations.
-  Local Open Scope string_scope.
-  Local Open Scope Z_scope.
-  Local Open Scope list_scope.
-
-  Context (F_add_func : (list string * list string * Syntax.cmd))
-          (F_copy_func : (list string * list string * Syntax.cmd))
-          (F_sub_func : (list string * list string * Syntax.cmd))
-          (F_select_znz_func : (list string * list string * Syntax.cmd))
-          (F_mul_func : (list string * list string * Syntax.cmd)).
-  
-  Definition F_add : bedrock2.Syntax.func := (@add F_names, F_add_func).
-
-  Definition F_copy : bedrock2.Syntax.func := (@felem_copy F_names, F_copy_func).
-
-  Definition F_mul : bedrock2.Syntax.func := (@mul F_names, F_mul_func).
-
-  Definition F_sub : bedrock2.Syntax.func := (@sub F_names, F_sub_func).
-
-  Definition F_select_znz : bedrock2.Syntax.func := (@select_znz F_names, F_select_znz_func).
-
-  (* Context {Fp2_names : FieldNames}. *)
-  Instance spec_of_add : spec_of (@add F_names).
-  Proof.
-    pose proof (@binop_spec width BW word mem locals ext_spec F _ _ add bin_add). cbv [spec_of]. eapply X.
-  Defined.
-
-  Instance spec_of_F_copy : spec_of (@felem_copy F_names).
-  Proof.
-    exact (spec_of_felem_copy (F:=F)).
-  Defined.
-
-  Instance spec_of_F_mul : spec_of (@mul F_names).
-  Proof.
-    pose proof (@binop_spec width BW word mem locals ext_spec F _ _ mul bin_mul).
-    cbv [spec_of]. apply X.
-  Defined.
-
-  Instance spec_of_F_sub : spec_of (@sub F_names).
-  Proof.
-    pose proof (@binop_spec width BW word mem locals ext_spec F _ _ sub bin_sub).
-    cbv [spec_of]. apply X.
-  Defined.
-
-  Instance spec_of_F_select_znz : spec_of (@select_znz F_names).
-  Proof.
-    pose proof (@spec_of_selectznz width BW word mem locals ext_spec F _ _ _). apply X.
-  Defined.
-
-  Check felem_offset.
-
   Definition expr_2nd_felem (x : Syntax.expr) := expr.op bopname.add x (expr.literal felem_offset).
 
-  Context (Fp2_names : FieldNames).
+  Context {Fp2_names : FieldNames Fp2}.
 
   Definition Fp2_select_znz : bedrock2.Syntax.func :=
-    (@Field.select_znz Fp2_names, (["out"; "c"; "inx"; "iny"], []:list String.string, bedrock_func_body:(
-       stackalloc (felem_size_in_bytes Fp2) as allocx;
-      stackalloc (felem_size_in_bytes Fp2) as allocy;
-      coq:(cmd.call [] (fst F_copy) [expr.var ("allocx"); expr.var ("inx")]);
-      coq:(cmd.call [] (fst F_copy) [expr_2nd_felem (expr.var ("allocx")); expr_2nd_felem (expr.var ("inx"))]);
-      coq:(cmd.call [] (fst F_copy) [expr.var ("allocy"); expr.var ("iny")]);
-      coq:(cmd.call [] (fst F_copy) [expr_2nd_felem (expr.var ("allocy")); expr_2nd_felem (expr.var ("iny"))]);
-      coq:(cmd.call [] ((fst F_select_znz)) [expr.var "out"; expr.var "c"; expr.var "allocx"; expr.var "allocy"]);
-      coq:(cmd.call [] ((fst F_select_znz)) [expr_2nd_felem (expr.var "out"); expr.var "c"; expr_2nd_felem (expr.var "allocx"); expr_2nd_felem (expr.var "allocy")])
-    ))).
-
-  Instance spec_of_Fp2_select_znz : spec_of (@Field.select_znz Fp2_names).
-  Proof.
-    simpl.
-    pose proof (@spec_of_selectznz width BW word mem locals ext_spec Fp2 Fp2_parameters Fp2_names Fp2_representation). eapply X.
-  Defined.
-
-  Definition Fp2_add : bedrock2.Syntax.func :=
-    (@Field.add Fp2_names, (["out"; "inx"; "iny"], []:list String.string, bedrock_func_body:(
+    (select_znz (F:=Fp2), (["out"; "c"; "inx"; "iny"], []:list String.string, bedrock_func_body:(
       stackalloc (felem_size_in_bytes Fp2) as allocx;
       stackalloc (felem_size_in_bytes Fp2) as allocy;
-      coq:(cmd.call [] (fst F_copy) [expr.var ("allocx"); expr.var ("inx")]);
-      coq:(cmd.call [] (fst F_copy) [expr_2nd_felem (expr.var ("allocx")); expr_2nd_felem (expr.var ("inx"))]);
-      coq:(cmd.call [] (fst F_copy) [expr.var ("allocy"); expr.var ("iny")]);
-      coq:(cmd.call [] (fst F_copy) [expr_2nd_felem (expr.var ("allocy")); expr_2nd_felem (expr.var ("iny"))]);
-      coq:(cmd.call [] ((fst F_add)) [expr.var "out"; expr.var "allocx"; expr.var "allocy"]);
-      coq:(cmd.call [] ((fst F_add)) [expr_2nd_felem (expr.var "out"); expr_2nd_felem (expr.var "allocx"); expr_2nd_felem (expr.var "allocy")])
+      coq:(cmd.call [] (felem_copy (F:=F)) [expr.var ("allocx"); expr.var ("inx")]);
+      coq:(cmd.call [] (felem_copy (F:=F)) [expr_2nd_felem (expr.var ("allocx")); expr_2nd_felem (expr.var ("inx"))]);
+      coq:(cmd.call [] (felem_copy (F:=F)) [expr.var ("allocy"); expr.var ("iny")]);
+      coq:(cmd.call [] (felem_copy (F:=F)) [expr_2nd_felem (expr.var ("allocy")); expr_2nd_felem (expr.var ("iny"))]);
+      coq:(cmd.call [] (select_znz (F:=F)) [expr.var "out"; expr.var "c"; expr.var "allocx"; expr.var "allocy"]);
+      coq:(cmd.call [] (select_znz (F:=F)) [expr_2nd_felem (expr.var "out"); expr.var "c"; expr_2nd_felem (expr.var "allocx"); expr_2nd_felem (expr.var "allocy")])
     ))).
 
-    Instance spec_of_Fp2_add : spec_of (@Field.add Fp2_names).
-    Proof.
-      simpl.
-      pose proof (@binop_spec width BW word mem locals ext_spec Fp2 _ _ (@Field.add Fp2_names) bin_add). cbv [spec_of]. eapply X.
-    Defined.
+  Instance spec_of_Fp2_select_znz : spec_of (select_znz (F:=Fp2)) := spec_of_selectznz (F:=Fp2).
 
-    Ltac bind_body_of_function' f := (*using alternative bind_body that does not normalize body of funcction, as it is horribly slow.*)
-      let fname := open_constr:(_) in
-      let fargs := open_constr:(_) in
-      let frets := open_constr:(_) in
-      let fbody := open_constr:(_) in
-      let funif := open_constr:((fname, (fargs, frets, fbody))) in
-      unify f funif;
-      let G := lazymatch goal with |- ?G => G end in
-      let P := lazymatch eval pattern f in G with ?P _ => P end in
-      change (bindcmd fbody (fun c : Syntax.cmd => P (fname, (fargs, frets, c))));
-      cbv beta iota delta [bindcmd]; intros.
+  Definition Fp2_add : bedrock2.Syntax.func :=
+    (add (F:=Fp2), (["out"; "inx"; "iny"], []:list String.string, bedrock_func_body:(
+      stackalloc (felem_size_in_bytes Fp2) as allocx;
+      stackalloc (felem_size_in_bytes Fp2) as allocy;
+      coq:(cmd.call [] (felem_copy (F:=F)) [expr.var ("allocx"); expr.var ("inx")]);
+      coq:(cmd.call [] (felem_copy (F:=F)) [expr_2nd_felem (expr.var ("allocx")); expr_2nd_felem (expr.var ("inx"))]);
+      coq:(cmd.call [] (felem_copy (F:=F)) [expr.var ("allocy"); expr.var ("iny")]);
+      coq:(cmd.call [] (felem_copy (F:=F)) [expr_2nd_felem (expr.var ("allocy")); expr_2nd_felem (expr.var ("iny"))]);
+      coq:(cmd.call [] (add (F:=F)) [expr.var "out"; expr.var "allocx"; expr.var "allocy"]);
+      coq:(cmd.call [] (add (F:=F)) [expr_2nd_felem (expr.var "out"); expr_2nd_felem (expr.var "allocx"); expr_2nd_felem (expr.var "allocy")])
+    ))).
+
+  Instance spec_of_Fp2_add : spec_of (add (F:=Fp2)) := binop_spec bin_add (F:=Fp2).
+
+  Ltac bind_body_of_function' f := (*using alternative bind_body that does not normalize body of funcction, as it is horribly slow.*)
+    let fname := open_constr:(_) in
+    let fargs := open_constr:(_) in
+    let frets := open_constr:(_) in
+    let fbody := open_constr:(_) in
+    let funif := open_constr:((fname, (fargs, frets, fbody))) in
+    unify f funif;
+    let G := lazymatch goal with |- ?G => G end in
+    let P := lazymatch eval pattern f in G with ?P _ => P end in
+    change (bindcmd fbody (fun c : Syntax.cmd => P (fname, (fargs, frets, c))));
+             cbv beta iota delta [bindcmd]; intros.
 
   Ltac enter' f :=
   cbv beta delta [program_logic_goal_for]; intros;
@@ -396,161 +326,163 @@ Section Fp2.
       repeat (erewrite map.get_put_diff; [| intros contra; discriminate]); eapply map.get_put_same|
     ]); repeat straightline.
 
-    Lemma Fp2_select_znz_ok : program_logic_goal_for_function! Fp2_select_znz.
-    Proof.
-      enter' Fp2_select_znz. clear H0 H1 H2. cbv [spec_of_selectznz] in *.
-      intros. unfold1_call_goal. cbv match beta delta [call_body].
-      assert ((select_znz =? select_znz)%string = true) by (rewrite eqb_refl; auto).
-      rewrite H1.
-      cbv match beta delta [func].
-      repeat straightline.
+  Import Syntax BinInt String List.ListNotations.
+
+  Lemma Fp2_select_znz_ok : program_logic_goal_for_function! Fp2_select_znz.
+  Proof.
+    enter' Fp2_select_znz. clear H0 H1 H2. cbv [spec_of_selectznz] in *.
+    intros. unfold1_call_goal. cbv match beta delta [call_body].
+    assert ((select_znz =? select_znz)%string = true) by (rewrite eqb_refl; auto).
+    rewrite H1.
+    cbv match beta delta [func].
+    repeat straightline.
 
     eapply Fp2_FElem_to_Fp_R_sep in H0.
     eapply Fp2_FElem_to_Fp_R_sep in H2.
     eapply Fp2_FElem_to_Fp_R_sep in H5.
 
-      collect H0 H2.
-      collect Hnew H5.
+    collect H0 H2.
+    collect Hnew H5.
 
-      split; [eapply felem_size_in_bytes_mod |].
-      repeat straightline.
-      split; [eapply felem_size_in_bytes_mod |].
-      repeat straightline.
-      eexists; split; [solve_locals l1 l0 l| ].
-      
-      eapply alloc_to_FElem in H5. destruct H5.
-      eapply alloc_to_FElem in H0. destruct H0.
-      eapply Fp2_FElem_to_Fp_sep in H0, H5.
-      eassert (((_ * _) * _)%sep mCombined0).
-      {
-        do 2 eexists; split; [eauto |]; split; [| apply H5].
-        do 2 eexists; split; [eauto |]; split; [| apply H0].
-        apply Hnew0.
-      }
-      clear dependent mStack.
-      clear dependent mStack0.
+    split; [eapply felem_size_in_bytes_mod |].
+    repeat straightline.
+    split; [eapply felem_size_in_bytes_mod |].
+    repeat straightline.
+    eexists; split; [solve_locals l1 l0 l| ].
 
-      straightline_call.
-      1: {
-        split; try ecancel_assumption.
-        remember ((Field.FElem _ a (fst_felem x1))) as R1.
-        remember (Field.FElem _ (word.add a felem_offset_word) (snd_felem x1)) as R2.
-        remember ((Field.FElem _ a0 (fst_felem x0))) as R3.
-        remember (Field.FElem _ (word.add a0 felem_offset_word) (snd_felem x0)) as R4.
-        remember (R1 * R2)%sep as R1'.
-        remember (R3 * R4)%sep as R2'.
-        eapply sep_assoc in H8.
+    eapply alloc_to_FElem in H5. destruct H5.
+    eapply alloc_to_FElem in H0. destruct H0.
+    eapply Fp2_FElem_to_Fp_sep in H0, H5.
+    eassert (((_ * _) * _)%sep mCombined0).
+    {
+      do 2 eexists; split; [eauto |]; split; [| apply H5].
+      do 2 eexists; split; [eauto |]; split; [| apply H0].
+      apply Hnew0.
+    }
+    clear dependent mStack.
+    clear dependent mStack0.
 
-        eapply sep_and_l_fwd in H8; destruct H8 as [H8 ?].
-        eapply sep_and_l_fwd in H8; destruct H8 as [H8 ?].
-        subst.
-        ecancel_assumption.
-      }
-      repeat straightline.
-      eexists; split; [solve_locals l1 l0 l| ].
+    straightline_call.
+    1: {
+      split; try ecancel_assumption.
+      remember ((Field.FElem _ a (fst_felem x1))) as R1.
+      remember (Field.FElem _ (word.add a felem_offset_word) (snd_felem x1)) as R2.
+      remember ((Field.FElem _ a0 (fst_felem x0))) as R3.
+      remember (Field.FElem _ (word.add a0 felem_offset_word) (snd_felem x0)) as R4.
+      remember (R1 * R2)%sep as R1'.
+      remember (R3 * R4)%sep as R2'.
+      eapply sep_assoc in H8.
 
-      straightline_call.
-      1: {
-        split; try ecancel_assumption.
-        cbv [id] in *.
-        remember ((Field.FElem _ a (fst_felem x))) as R1.
-        remember (Field.FElem _ (word.add a felem_offset_word) (snd_felem x1)) as R2.
-        remember ((Field.FElem _ a0 (fst_felem x0))) as R3.
-        remember (Field.FElem _ (word.add a0 felem_offset_word) (snd_felem x0)) as R4.
-        eapply sep_comm in H5.
-        eapply sep_assoc in H5.
-        remember (R2 * (R3 * R4) * R1)%sep as R1'.
-        eapply sep_and_l_fwd in H5; destruct H5 as [H5 ?].
-        eapply sep_and_l_fwd in H5; destruct H5 as [H5 ?].
-        subst.
-        ecancel_assumption.
-      }
-      repeat straightline.
-      eexists; split; [solve_locals l1 l0 l| ].
+      eapply sep_and_l_fwd in H8; destruct H8 as [H8 ?].
+      eapply sep_and_l_fwd in H8; destruct H8 as [H8 ?].
+      subst.
+      ecancel_assumption.
+    }
+    repeat straightline.
+    eexists; split; [solve_locals l1 l0 l| ].
 
-      straightline_call.
-      1: {
-        split; try ecancel_assumption.
-        cbv [id] in *.
-        remember ((Field.FElem _ a (fst_felem x))) as R1.
-        remember (Field.FElem _ (word.add a felem_offset_word) (snd_felem x)) as R2.
-        remember ((Field.FElem _ a0 (fst_felem x0))) as R3.
-        remember (Field.FElem _ (word.add a0 felem_offset_word) (snd_felem x0)) as R4.
-        eapply sep_comm in H7.
-        eapply sep_assoc in H7.
-        eapply sep_comm in H7.
-        eapply sep_assoc in H7.
-        remember ((R3 * R4))%sep as R1'.
-        remember ((R2 * R1))%sep as R2'.
-        eapply sep_assoc in H7.
-        eapply sep_and_l_fwd in H7; destruct H7 as [H7 ?].
-        eapply sep_and_l_fwd in H7; destruct H7 as [H7 ?].
-        subst.
-        ecancel_assumption.
-      }
+    straightline_call.
+    1: {
+      split; try ecancel_assumption.
+      cbv [id] in *.
+      remember ((Field.FElem _ a (fst_felem x))) as R1.
+      remember (Field.FElem _ (word.add a felem_offset_word) (snd_felem x1)) as R2.
+      remember ((Field.FElem _ a0 (fst_felem x0))) as R3.
+      remember (Field.FElem _ (word.add a0 felem_offset_word) (snd_felem x0)) as R4.
+      eapply sep_comm in H5.
+      eapply sep_assoc in H5.
+      remember (R2 * (R3 * R4) * R1)%sep as R1'.
+      eapply sep_and_l_fwd in H5; destruct H5 as [H5 ?].
+      eapply sep_and_l_fwd in H5; destruct H5 as [H5 ?].
+      subst.
+      ecancel_assumption.
+    }
+    repeat straightline.
+    eexists; split; [solve_locals l1 l0 l| ].
 
-      repeat straightline.
-      eexists; split; [solve_locals l1 l0 l| ].
+    straightline_call.
+    1: {
+      split; try ecancel_assumption.
+      cbv [id] in *.
+      remember ((Field.FElem _ a (fst_felem x))) as R1.
+      remember (Field.FElem _ (word.add a felem_offset_word) (snd_felem x)) as R2.
+      remember ((Field.FElem _ a0 (fst_felem x0))) as R3.
+      remember (Field.FElem _ (word.add a0 felem_offset_word) (snd_felem x0)) as R4.
+      eapply sep_comm in H7.
+      eapply sep_assoc in H7.
+      eapply sep_comm in H7.
+      eapply sep_assoc in H7.
+      remember ((R3 * R4))%sep as R1'.
+      remember ((R2 * R1))%sep as R2'.
+      eapply sep_assoc in H7.
+      eapply sep_and_l_fwd in H7; destruct H7 as [H7 ?].
+      eapply sep_and_l_fwd in H7; destruct H7 as [H7 ?].
+      subst.
+      ecancel_assumption.
+    }
 
-      straightline_call.
-      1: {
-        split; try ecancel_assumption.
-        cbv [id] in *.
-        remember ((Field.FElem _ a (fst_felem x))) as R1.
-        remember (Field.FElem _ (word.add a felem_offset_word) (snd_felem x)) as R2.
-        remember ((Field.FElem _ a0 (fst_felem y))) as R3.
-        remember (Field.FElem _ (word.add a0 felem_offset_word) (snd_felem x0)) as R4.
-        eapply sep_comm in H9.
-        eapply sep_assoc in H9.
-        eapply sep_comm in H9.
-        eapply sep_assoc in H9.
-        eapply (sep_assoc _ _ (R3 * R2)%sep) in H9.
-        eapply (sep_comm R1) in H9.
-        eapply sep_assoc in H9.
-        remember ((R3 * R2 * R1))%sep as R1'.
-        eapply sep_assoc in H9.
-        eapply sep_and_l_fwd in H9; destruct H9 as [H9 ?].
-        eapply sep_and_l_fwd in H9; destruct H9 as [H9 ?].
-        subst.
-        ecancel_assumption.
-      }
+    repeat straightline.
+    eexists; split; [solve_locals l1 l0 l| ].
 
-      repeat straightline.
-      eexists; split; [solve_locals l1 l0 l |].
-
-      (*deconstructing sep hyp.*)
+    straightline_call.
+    1: {
+      split; try ecancel_assumption.
       cbv [id] in *.
       remember ((Field.FElem _ a (fst_felem x))) as R1.
       remember (Field.FElem _ (word.add a felem_offset_word) (snd_felem x)) as R2.
       remember ((Field.FElem _ a0 (fst_felem y))) as R3.
-      remember (Field.FElem _ (word.add a0 felem_offset_word) (snd_felem y)) as R4.
-      rename H10 into H11.
-      eapply sep_assoc in H11. eapply (sep_assoc (R4 * R3)%sep) in H11.
-      eapply (sep_assoc (R4 * R3 * R2)%sep) in H11.
-      eapply sep_comm in H11.
-      eapply sep_and_l_fwd in H11; destruct H11 as [H11 ?].
-      eapply sep_and_l_fwd in H11; destruct H11 as [H11 ?].
+      remember (Field.FElem _ (word.add a0 felem_offset_word) (snd_felem x0)) as R4.
+      eapply sep_comm in H9.
+      eapply sep_assoc in H9.
+      eapply sep_comm in H9.
+      eapply sep_assoc in H9.
+      eapply (sep_assoc _ _ (R3 * R2)%sep) in H9.
+      eapply (sep_comm R1) in H9.
+      eapply sep_assoc in H9.
+      remember ((R3 * R2 * R1))%sep as R1'.
+      eapply sep_assoc in H9.
+      eapply sep_and_l_fwd in H9; destruct H9 as [H9 ?].
+      eapply sep_and_l_fwd in H9; destruct H9 as [H9 ?].
       subst.
+      ecancel_assumption.
+    }
 
-      straightline_call.
+    repeat straightline.
+    eexists; split; [solve_locals l1 l0 l |].
+
+    (*deconstructing sep hyp.*)
+    cbv [id] in *.
+    remember ((Field.FElem _ a (fst_felem x))) as R1.
+    remember (Field.FElem _ (word.add a felem_offset_word) (snd_felem x)) as R2.
+    remember ((Field.FElem _ a0 (fst_felem y))) as R3.
+    remember (Field.FElem _ (word.add a0 felem_offset_word) (snd_felem y)) as R4.
+    rename H10 into H11.
+    eapply sep_assoc in H11. eapply (sep_assoc (R4 * R3)%sep) in H11.
+    eapply (sep_assoc (R4 * R3 * R2)%sep) in H11.
+    eapply sep_comm in H11.
+    eapply sep_and_l_fwd in H11; destruct H11 as [H11 ?].
+    eapply sep_and_l_fwd in H11; destruct H11 as [H11 ?].
+    subst.
+
+    straightline_call.
+    1: {
+      split; [| split; [| split]].
       1: {
-        split; [| split; [| split]].
-        1: {
-          subst. ecancel_assumption.
-        }
-        2: {
-          subst. clear H2 H0. ecancel_assumption.
-        }
-        1: { subst. clear H2 H0. ecancel_assumption.
-        }
-        auto.
+        subst. ecancel_assumption.
       }
+      2: {
+        subst. clear H2 H0. ecancel_assumption.
+      }
+      1: { subst. clear H2 H0. ecancel_assumption.
+      }
+      auto.
+    }
 
-      repeat straightline.
-      eexists; split; [solve_locals l1 l0 l| ].
-      destruct (word.unsigned pc =? 1) eqn:eq.
-      (*after destruct*)
-      {
+    repeat straightline.
+    eexists; split; [solve_locals l1 l0 l| ].
+    destruct (word.unsigned pc =? 1) eqn:eq.
+    (*after destruct*)
+    {
 
       straightline_call.
       1: {
@@ -561,12 +493,9 @@ Section Fp2.
         1: auto.
       }
 
-
-      
       repeat straightline. (*mStack is not in scope in the below proof; should otherwise go through. destruct sep hyp before introducing evars.*)
 
       rewrite eq in H16.
-
 
       eassert ((Field.FElem _ a0 _  * _)%sep a8).
       {
@@ -597,249 +526,44 @@ Section Fp2.
       split; [eapply map.split_comm; eauto| ].
 
       repeat straightline. split; auto. 
-        eapply Fp_FElem_to_Fp2_R_sep.
-        ecancel_assumption.
-      }
-      (*other case for conditional*)
-      {
-        straightline_call.
-        1: {
-          split; [| split; [| split]].
-          1: subst; ecancel_assumption.
-          1: subst; ecancel_assumption.
-          1: subst; ecancel_assumption.
-          1: auto.
-        }
-  
-  
-        
-        repeat straightline. (*mStack is not in scope in the below proof; should otherwise go through. destruct sep hyp before introducing evars.*)
-  
-        rewrite eq in H16.
-  
-  
-        eassert ((Field.FElem _ a0 _  * _)%sep a8).
-        {
-          eapply Fp_FElem_to_Fp2_R_sep. ecancel_assumption.
-        }
-        destruct H10, H10, H10, H17.
-        eexists. eexists. split.
-        1: {
-          eapply FElem_Fp2_to_anybytes. eauto.
-        }
-        split; [eapply map.split_comm; eauto| ].
-  
-        clear H16 H12 H5 H0 H2 H11 H9 H7 H13 H14.
-  
-        eassert ((Field.FElem _ a _  * _)%sep x3).
-        {
-          eapply Fp_FElem_to_Fp2_R_sep. ecancel_assumption.
-        }
-        clear H18.
-  
-        destruct H0, H0, H0, H2.
-  
-        do 2 eexists; split.
-        1: {
-          eapply FElem_Fp2_to_anybytes; eauto.
-        }
-  
-        split; [eapply map.split_comm; eauto| ].
-  
-        repeat straightline. split; auto. 
-          eapply Fp_FElem_to_Fp2_R_sep.
-          ecancel_assumption.
-      }
-    Qed.
-    (*Proof of select_znz_Fp2 finished.*)
-
-
-    Lemma Fp2_add_ok : program_logic_goal_for_function! Fp2_add.
-    Proof.
-      enter' Fp2_add. clear H0 H1 H2. cbv [binop_spec] in *.
-      intros. unfold1_call_goal. cbv match beta delta [call_body].
-      assert ((Field.add =? Field.add)%string = true) by (rewrite eqb_refl; auto).
-      rewrite H1.
-      cbv match beta delta [func].
-      repeat straightline.
-
-    eapply Fp2_FElem_to_Fp_R_sep in H5, H6, H7.
-
-      collect H5 H6.
-      collect Hnew H7.
-
-      split; [eapply felem_size_in_bytes_mod |].
-      repeat straightline.
-      split; [eapply felem_size_in_bytes_mod |].
-      repeat straightline.
-      eexists; split; [solve_locals l1 l0 l| ].
-      
-      eapply alloc_to_FElem in H7. destruct H7.
-      eapply alloc_to_FElem in H5. destruct H5.
-      eapply Fp2_FElem_to_Fp_sep in H5, H7.
-      eassert (((_ * _) * _)%sep mCombined0).
-      {
-        do 2 eexists; split; [eauto |]; split; [| apply H7].
-        do 2 eexists; split; [eauto |]; split; [| apply H5].
-        apply Hnew0.
-      }
-      clear dependent mStack.
-      clear dependent mStack0.
-
+      eapply Fp_FElem_to_Fp2_R_sep.
+      ecancel_assumption.
+    }
+    (*other case for conditional*)
+    {
       straightline_call.
       1: {
-        split; try ecancel_assumption.
-        remember ((Field.FElem _ a (fst_felem x3))) as R1.
-        remember (Field.FElem _ (word.add a felem_offset_word) (snd_felem x3)) as R2.
-        remember ((Field.FElem _ a0 (fst_felem x2))) as R3.
-        remember (Field.FElem _ (word.add a0 felem_offset_word) (snd_felem x2)) as R4.
-        remember (R1 * R2)%sep as R1'.
-        remember (R3 * R4)%sep as R2'.
-        eapply sep_assoc in H9.
-
-        eapply sep_and_l_fwd in H9; destruct H9 as [H9 ?].
-        eapply sep_and_l_fwd in H9; destruct H9 as [H9 ?].
-        subst.
-        ecancel_assumption.
-      }
-      repeat straightline.
-      eexists; split; [solve_locals l1 l0 l| ].
-
-      straightline_call.
-      1: {
-        split; try ecancel_assumption.
-        cbv [id] in *.
-        remember ((Field.FElem _ a (fst_felem x))) as R1.
-        remember (Field.FElem _ (word.add a felem_offset_word) (snd_felem x3)) as R2.
-        remember ((Field.FElem _ a0 (fst_felem x2))) as R3.
-        remember (Field.FElem _ (word.add a0 felem_offset_word) (snd_felem x2)) as R4.
-        eapply sep_comm in H7.
-        eapply sep_assoc in H7.
-        remember (R2 * (R3 * R4) * R1)%sep as R1'.
-        eapply sep_and_l_fwd in H7; destruct H7 as [H7 ?].
-        eapply sep_and_l_fwd in H7; destruct H7 as [H7 ?].
-        subst.
-        ecancel_assumption.
-      }
-      repeat straightline.
-      eexists; split; [solve_locals l1 l0 l| ].
-
-      straightline_call.
-      1: {
-        split; try ecancel_assumption.
-        cbv [id] in *.
-        remember ((Field.FElem _ a (fst_felem x))) as R1.
-        remember (Field.FElem _ (word.add a felem_offset_word) (snd_felem x)) as R2.
-        remember ((Field.FElem _ a0 (fst_felem x2))) as R3.
-        remember (Field.FElem _ (word.add a0 felem_offset_word) (snd_felem x2)) as R4.
-        eapply sep_comm in H8.
-        eapply sep_assoc in H8.
-        eapply sep_comm in H8.
-        eapply sep_assoc in H8.
-        remember ((R3 * R4))%sep as R1'.
-        remember ((R2 * R1))%sep as R2'.
-        eapply sep_assoc in H8.
-        eapply sep_and_l_fwd in H8; destruct H8 as [H8 ?].
-        eapply sep_and_l_fwd in H8; destruct H8 as [H8 ?].
-        subst.
-        ecancel_assumption.
-      }
-
-      repeat straightline.
-      eexists; split; [solve_locals l1 l0 l| ].
-
-      straightline_call.
-      1: {
-        split; try ecancel_assumption.
-        cbv [id] in *.
-        remember ((Field.FElem _ a (fst_felem x))) as R1.
-        remember (Field.FElem _ (word.add a felem_offset_word) (snd_felem x)) as R2.
-        remember ((Field.FElem _ a0 (fst_felem y))) as R3.
-        remember (Field.FElem _ (word.add a0 felem_offset_word) (snd_felem x2)) as R4.
-        eapply sep_comm in H10.
-        eapply sep_assoc in H10.
-        eapply sep_comm in H10.
-        eapply sep_assoc in H10.
-        eapply (sep_assoc _ _ (R3 * R2)%sep) in H10.
-        eapply (sep_comm R1) in H10.
-        eapply sep_assoc in H10.
-        remember ((R3 * R2 * R1))%sep as R1'.
-        eapply sep_assoc in H10.
-        eapply sep_and_l_fwd in H10; destruct H10 as [H10 ?].
-        eapply sep_and_l_fwd in H10; destruct H10 as [H10 ?].
-        subst.
-        ecancel_assumption.
-      }
-
-      repeat straightline.
-      eexists; split; [solve_locals l1 l0 l |].
-
-      (*deconstructing sep hyp.*)
-      cbv [id] in *.
-      remember ((Field.FElem _ a (fst_felem x))) as R1.
-      remember (Field.FElem _ (word.add a felem_offset_word) (snd_felem x)) as R2.
-      remember ((Field.FElem _ a0 (fst_felem y))) as R3.
-      remember (Field.FElem _ (word.add a0 felem_offset_word) (snd_felem y)) as R4.
-      eapply sep_assoc in H11. eapply (sep_assoc (R4 * R3)%sep) in H11.
-      eapply (sep_assoc (R4 * R3 * R2)%sep) in H11.
-      eapply sep_comm in H11.
-      eapply sep_and_l_fwd in H11; destruct H11 as [H11 ?].
-      clear H11. subst.
-
-
-      straightline_call.
-      1: {
-        split; [|split; [| split; [| split]]].
-        5: {
-          subst; ecancel_assumption.
-        }
-        3: {
-          eexists. ecancel_assumption.
-        }
-        3: {
-          eexists; ecancel_assumption.
-        }
-        1: {
-          destruct H0. eauto.
-        }
-        1: {
-          destruct H2; eauto.
-        }
-      }
-      repeat straightline.
-      eexists; split; [solve_locals l1 l0 l| ].
-
-      straightline_call.
-      1: {
-        split; [| split; [| split; [| split]]].
-        5: ecancel_assumption.
-        4: eexists; ecancel_assumption.
-        3: eexists; ecancel_assumption.
-        1: destruct H0; eauto.
-        1: destruct H2; eauto.
+        split; [| split; [| split]].
+        1: subst; ecancel_assumption.
+        1: subst; ecancel_assumption.
+        1: subst; ecancel_assumption.
+        1: auto.
       }
 
       repeat straightline. (*mStack is not in scope in the below proof; should otherwise go through. destruct sep hyp before introducing evars.*)
+
+      rewrite eq in H16.
+
       eassert ((Field.FElem _ a0 _  * _)%sep a8).
       {
         eapply Fp_FElem_to_Fp2_R_sep. ecancel_assumption.
       }
-      destruct H6, H6, H6, H11.
+      destruct H10, H10, H10, H17.
       eexists. eexists. split.
       1: {
         eapply FElem_Fp2_to_anybytes. eauto.
       }
       split; [eapply map.split_comm; eauto| ].
 
-      clear H20 H14 H5 H10 H8 H7 H9.
+      clear H16 H12 H5 H0 H2 H11 H9 H7 H13 H14.
 
-      eassert ((Field.FElem _ a _  * _)%sep x7).
+      eassert ((Field.FElem _ a _  * _)%sep x3).
       {
         eapply Fp_FElem_to_Fp2_R_sep. ecancel_assumption.
       }
-      clear H21.
+      clear H18.
 
-      destruct H5, H5, H5, H7.
+      destruct H0, H0, H0, H2.
 
       do 2 eexists; split.
       1: {
@@ -848,439 +572,631 @@ Section Fp2.
 
       split; [eapply map.split_comm; eauto| ].
 
-      repeat straightline. split; auto. split; auto.
+      repeat straightline. split; auto.
+      eapply Fp_FElem_to_Fp2_R_sep.
+      ecancel_assumption.
+    }
+  Qed.
+  (*Proof of select_znz_Fp2 finished.*)
 
-      exists (x4 ++ x5). split; [| split].
+  Lemma Fp2_add_ok : program_logic_goal_for_function! Fp2_add.
+  Proof.
+    enter' Fp2_add. clear H0 H1 H2. cbv [binop_spec] in *.
+    intros. unfold1_call_goal. cbv match beta delta [call_body].
+    assert ((Field.add =? Field.add)%string = true) by (rewrite eqb_refl; auto).
+    rewrite H1.
+    cbv match beta delta [func].
+    repeat straightline.
 
+    eapply Fp2_FElem_to_Fp_R_sep in H5, H6, H7.
+
+    collect H5 H6.
+    collect Hnew H7.
+
+    split; [eapply felem_size_in_bytes_mod |].
+    repeat straightline.
+    split; [eapply felem_size_in_bytes_mod |].
+    repeat straightline.
+    eexists; split; [solve_locals l1 l0 l| ].
+
+    eapply alloc_to_FElem in H7. destruct H7.
+    eapply alloc_to_FElem in H5. destruct H5.
+    eapply Fp2_FElem_to_Fp_sep in H5, H7.
+    eassert (((_ * _) * _)%sep mCombined0).
+    {
+      do 2 eexists; split; [eauto |]; split; [| apply H7].
+      do 2 eexists; split; [eauto |]; split; [| apply H5].
+      apply Hnew0.
+    }
+    clear dependent mStack.
+    clear dependent mStack0.
+
+    straightline_call.
+    1: {
+      split; try ecancel_assumption.
+      remember ((Field.FElem _ a (fst_felem x3))) as R1.
+      remember (Field.FElem _ (word.add a felem_offset_word) (snd_felem x3)) as R2.
+      remember ((Field.FElem _ a0 (fst_felem x2))) as R3.
+      remember (Field.FElem _ (word.add a0 felem_offset_word) (snd_felem x2)) as R4.
+      remember (R1 * R2)%sep as R1'.
+      remember (R3 * R4)%sep as R2'.
+      eapply sep_assoc in H9.
+
+      eapply sep_and_l_fwd in H9; destruct H9 as [H9 ?].
+      eapply sep_and_l_fwd in H9; destruct H9 as [H9 ?].
+      subst.
+      ecancel_assumption.
+    }
+    repeat straightline.
+    eexists; split; [solve_locals l1 l0 l| ].
+
+    straightline_call.
+    1: {
+      split; try ecancel_assumption.
+      cbv [id] in *.
+      remember ((Field.FElem _ a (fst_felem x))) as R1.
+      remember (Field.FElem _ (word.add a felem_offset_word) (snd_felem x3)) as R2.
+      remember ((Field.FElem _ a0 (fst_felem x2))) as R3.
+      remember (Field.FElem _ (word.add a0 felem_offset_word) (snd_felem x2)) as R4.
+      eapply sep_comm in H7.
+      eapply sep_assoc in H7.
+      remember (R2 * (R3 * R4) * R1)%sep as R1'.
+      eapply sep_and_l_fwd in H7; destruct H7 as [H7 ?].
+      eapply sep_and_l_fwd in H7; destruct H7 as [H7 ?].
+      subst.
+      ecancel_assumption.
+    }
+    repeat straightline.
+    eexists; split; [solve_locals l1 l0 l| ].
+
+    straightline_call.
+    1: {
+      split; try ecancel_assumption.
+      cbv [id] in *.
+      remember ((Field.FElem _ a (fst_felem x))) as R1.
+      remember (Field.FElem _ (word.add a felem_offset_word) (snd_felem x)) as R2.
+      remember ((Field.FElem _ a0 (fst_felem x2))) as R3.
+      remember (Field.FElem _ (word.add a0 felem_offset_word) (snd_felem x2)) as R4.
+      eapply sep_comm in H8.
+      eapply sep_assoc in H8.
+      eapply sep_comm in H8.
+      eapply sep_assoc in H8.
+      remember ((R3 * R4))%sep as R1'.
+      remember ((R2 * R1))%sep as R2'.
+      eapply sep_assoc in H8.
+      eapply sep_and_l_fwd in H8; destruct H8 as [H8 ?].
+      eapply sep_and_l_fwd in H8; destruct H8 as [H8 ?].
+      subst.
+      ecancel_assumption.
+    }
+
+    repeat straightline.
+    eexists; split; [solve_locals l1 l0 l| ].
+
+    straightline_call.
+    1: {
+      split; try ecancel_assumption.
+      cbv [id] in *.
+      remember ((Field.FElem _ a (fst_felem x))) as R1.
+      remember (Field.FElem _ (word.add a felem_offset_word) (snd_felem x)) as R2.
+      remember ((Field.FElem _ a0 (fst_felem y))) as R3.
+      remember (Field.FElem _ (word.add a0 felem_offset_word) (snd_felem x2)) as R4.
+      eapply sep_comm in H10.
+      eapply sep_assoc in H10.
+      eapply sep_comm in H10.
+      eapply sep_assoc in H10.
+      eapply (sep_assoc _ _ (R3 * R2)%sep) in H10.
+      eapply (sep_comm R1) in H10.
+      eapply sep_assoc in H10.
+      remember ((R3 * R2 * R1))%sep as R1'.
+      eapply sep_assoc in H10.
+      eapply sep_and_l_fwd in H10; destruct H10 as [H10 ?].
+      eapply sep_and_l_fwd in H10; destruct H10 as [H10 ?].
+      subst.
+      ecancel_assumption.
+    }
+
+    repeat straightline.
+    eexists; split; [solve_locals l1 l0 l |].
+
+    (*deconstructing sep hyp.*)
+    cbv [id] in *.
+    remember ((Field.FElem _ a (fst_felem x))) as R1.
+    remember (Field.FElem _ (word.add a felem_offset_word) (snd_felem x)) as R2.
+    remember ((Field.FElem _ a0 (fst_felem y))) as R3.
+    remember (Field.FElem _ (word.add a0 felem_offset_word) (snd_felem y)) as R4.
+    eapply sep_assoc in H11. eapply (sep_assoc (R4 * R3)%sep) in H11.
+    eapply (sep_assoc (R4 * R3 * R2)%sep) in H11.
+    eapply sep_comm in H11.
+    eapply sep_and_l_fwd in H11; destruct H11 as [H11 ?].
+    clear H11. subst.
+
+
+    straightline_call.
+    1: {
+      split; [|split; [| split; [| split]]].
+      5: {
+        subst; ecancel_assumption.
+      }
       3: {
-        eapply Fp_FElem_to_Fp2_R_sep. erewrite fst_felem_app; [| ecancel_assumption].
-        erewrite snd_felem_app; [| ecancel_assumption].
-        ecancel_assumption.
+        eexists. ecancel_assumption.
       }
-      2: {
-        split; eauto. erewrite fst_felem_app; try ecancel_assumption; auto.
-        erewrite snd_felem_app; try ecancel_assumption; auto.
+      3: {
+        eexists; ecancel_assumption.
       }
-      simpl.
-      cbv [addp2].
-      apply Prod.path_pair.
       1: {
-        erewrite fst_felem_app; try ecancel_assumption. simpl. auto.
+        destruct H0. eauto.
       }
-      erewrite snd_felem_app; try ecancel_assumption; simpl; auto.
-    Qed.
+      1: {
+        destruct H2; eauto.
+      }
+    }
+    repeat straightline.
+    eexists; split; [solve_locals l1 l0 l| ].
 
-    (*multiplication in Fp2*)
+    straightline_call.
+    1: {
+      split; [| split; [| split; [| split]]].
+      5: ecancel_assumption.
+      4: eexists; ecancel_assumption.
+      3: eexists; ecancel_assumption.
+      1: destruct H0; eauto.
+      1: destruct H2; eauto.
+    }
 
-    Definition Fp2_mul : bedrock2.Syntax.func :=
-      (@Field.mul Fp2_names, (["out"; "inx"; "iny"], []:list String.string, bedrock_func_body:(
+    repeat straightline. (*mStack is not in scope in the below proof; should otherwise go through. destruct sep hyp before introducing evars.*)
+    eassert ((Field.FElem _ a0 _  * _)%sep a8).
+    {
+      eapply Fp_FElem_to_Fp2_R_sep. ecancel_assumption.
+    }
+    destruct H6, H6, H6, H11.
+    eexists. eexists. split.
+    1: {
+      eapply FElem_Fp2_to_anybytes. eauto.
+    }
+    split; [eapply map.split_comm; eauto| ].
+
+    clear H20 H14 H5 H10 H8 H7 H9.
+
+    eassert ((Field.FElem _ a _  * _)%sep x7).
+    {
+      eapply Fp_FElem_to_Fp2_R_sep. ecancel_assumption.
+    }
+    clear H21.
+
+    destruct H5, H5, H5, H7.
+
+    do 2 eexists; split.
+    1: {
+      eapply FElem_Fp2_to_anybytes; eauto.
+    }
+
+    split; [eapply map.split_comm; eauto| ].
+
+    repeat straightline. split; auto. split; auto.
+
+    exists (x4 ++ x5). split; [| split].
+
+    3: {
+      eapply Fp_FElem_to_Fp2_R_sep. erewrite fst_felem_app; [| ecancel_assumption].
+      erewrite snd_felem_app; [| ecancel_assumption].
+      ecancel_assumption.
+    }
+    2: {
+      split; eauto. erewrite fst_felem_app; try ecancel_assumption; auto.
+      erewrite snd_felem_app; try ecancel_assumption; auto.
+    }
+    simpl.
+    cbv [addp2].
+    apply Prod.path_pair.
+    1: {
+      erewrite fst_felem_app; try ecancel_assumption. simpl. auto.
+    }
+    erewrite snd_felem_app; try ecancel_assumption; simpl; auto.
+  Qed.
+
+  (*multiplication in Fp2*)
+
+  Definition Fp2_mul : bedrock2.Syntax.func :=
+    (mul (F:=Fp2), (["out"; "inx"; "iny"], []:list String.string, bedrock_func_body:(
         stackalloc (felem_size_in_bytes F) as v0;
         stackalloc (felem_size_in_bytes F) as v1;
         stackalloc (felem_size_in_bytes Fp2) as allocx;
         stackalloc (felem_size_in_bytes Fp2) as allocy;
-        coq:(cmd.call [] (fst F_copy) [expr.var ("allocx"); expr.var ("inx")]);
-        coq:(cmd.call [] (fst F_copy) [expr_2nd_felem (expr.var ("allocx")); expr_2nd_felem (expr.var ("inx"))]);
-        coq:(cmd.call [] (fst F_copy) [expr.var ("allocy"); expr.var ("iny")]);
-        coq:(cmd.call [] (fst F_copy) [expr_2nd_felem (expr.var ("allocy")); expr_2nd_felem (expr.var ("iny"))]);
-        coq:(cmd.call [] ((fst F_mul)) [expr.var "v0"; expr.var "allocx"; expr.var "allocy"]);
-        coq:(cmd.call [] ((fst F_mul)) [expr.var "v1"; expr_2nd_felem (expr.var "allocx"); expr_2nd_felem (expr.var "allocy")]);
-        coq:(cmd.call [] ((fst F_add)) [expr.var "out"; expr.var "allocx"; expr_2nd_felem (expr.var "allocx")]);
-        coq:(cmd.call [] ((fst F_add)) [expr_2nd_felem (expr.var "out"); expr.var "allocy"; expr_2nd_felem (expr.var "allocy")]);
-        coq:(cmd.call [] ((fst F_mul)) [expr_2nd_felem (expr.var "out"); expr_2nd_felem (expr.var "out"); expr.var "out"]);
-        coq:(cmd.call [] ((fst F_sub)) [expr_2nd_felem (expr.var "out"); expr_2nd_felem (expr.var "out"); expr.var "v0"]);
-        coq:(cmd.call [] ((fst F_sub)) [expr_2nd_felem (expr.var "out"); expr_2nd_felem (expr.var "out"); expr.var "v1"]);
-        coq:(cmd.call [] ((fst F_sub)) [expr.var "out"; expr.var "v0"; expr.var "v1"])
-      ))).
+        coq:(cmd.call [] (felem_copy (F:=F)) [expr.var ("allocx"); expr.var ("inx")]);
+        coq:(cmd.call [] (felem_copy (F:=F)) [expr_2nd_felem (expr.var ("allocx")); expr_2nd_felem (expr.var ("inx"))]);
+        coq:(cmd.call [] (felem_copy (F:=F)) [expr.var ("allocy"); expr.var ("iny")]);
+        coq:(cmd.call [] (felem_copy (F:=F)) [expr_2nd_felem (expr.var ("allocy")); expr_2nd_felem (expr.var ("iny"))]);
+        coq:(cmd.call [] (mul (F:=F)) [expr.var "v0"; expr.var "allocx"; expr.var "allocy"]);
+        coq:(cmd.call [] (mul (F:=F)) [expr.var "v1"; expr_2nd_felem (expr.var "allocx"); expr_2nd_felem (expr.var "allocy")]);
+        coq:(cmd.call [] (add (F:=F)) [expr.var "out"; expr.var "allocx"; expr_2nd_felem (expr.var "allocx")]);
+        coq:(cmd.call [] (add (F:=F)) [expr_2nd_felem (expr.var "out"); expr.var "allocy"; expr_2nd_felem (expr.var "allocy")]);
+        coq:(cmd.call [] (mul (F:=F)) [expr_2nd_felem (expr.var "out"); expr_2nd_felem (expr.var "out"); expr.var "out"]);
+        coq:(cmd.call [] (sub (F:=F)) [expr_2nd_felem (expr.var "out"); expr_2nd_felem (expr.var "out"); expr.var "v0"]);
+        coq:(cmd.call [] (sub (F:=F)) [expr_2nd_felem (expr.var "out"); expr_2nd_felem (expr.var "out"); expr.var "v1"]);
+        coq:(cmd.call [] (sub (F:=F)) [expr.var "out"; expr.var "v0"; expr.var "v1"])
+    ))).
 
-    Instance spec_of_Fp2_mul : spec_of (@Field.mul Fp2_names).
-    Proof.
-      simpl.
-      pose proof (@binop_spec width BW word mem locals ext_spec Fp2 Fp2_parameters Fp2_representation (@Field.mul Fp2_names) bin_mul). cbv [spec_of]. eapply X.
-    Defined.
+  Instance spec_of_Fp2_mul : spec_of (mul (F:=Fp2)) := binop_spec bin_mul (F:=Fp2).
 
-    Lemma M_pos_prime : Znumtheory.prime (Z.pos M_pos).
-    Proof.
-      destruct prime_parameters_ok; auto.
-    Qed.
+  Lemma M_pos_prime : Znumtheory.prime (Z.pos M_pos).
+  Proof.
+    destruct prime_parameters_ok; auto.
+  Qed.
 
-    Lemma Fp2_mul_ok : program_logic_goal_for_function! Fp2_mul.
-    Proof.
-      enter' Fp2_mul. clear H0 H1 H2 H3 H4 H5 H8 H9. cbv [binop_spec] in *.
-      intros. unfold1_call_goal. cbv match beta delta [call_body].
-      assert ((Field.mul =? Field.mul)%string = true) by (rewrite eqb_refl; auto).
-      rewrite H1.
-      cbv match beta delta [func].
-      repeat straightline.
+  Lemma Fp2_mul_ok : program_logic_goal_for_function! Fp2_mul.
+  Proof.
+    enter' Fp2_mul. clear H0 H1 H2 H3 H4 H5 H8 H9. cbv [binop_spec] in *.
+    intros. unfold1_call_goal. cbv match beta delta [call_body].
+    assert ((Field.mul =? Field.mul)%string = true) by (rewrite eqb_refl; auto).
+    rewrite H1.
+    cbv match beta delta [func].
+    repeat straightline.
 
     eapply Fp2_FElem_to_Fp_R_sep in H3, H4, H5.
 
-      collect H3 H4.
-      collect Hnew H5.
+    collect H3 H4.
+    collect Hnew H5.
 
-      split; [eapply felem_size_in_bytes_mod |].
-      repeat straightline.
-      split; [eapply felem_size_in_bytes_mod |].
-      repeat straightline.
-      split; [eapply felem_size_in_bytes_mod |].
-      repeat straightline.
-      split; [eapply felem_size_in_bytes_mod |].
-      repeat straightline.
-      eexists; split; [solve_locals5 l3 l2 l1 l0 l| ].
-      
-      eapply alloc_to_FElem in H9. destruct H9.
-      eapply alloc_to_FElem in H12. destruct H12.
-      eapply Fp2_FElem_to_Fp_sep in H9, H12.
-      eapply alloc_to_FElem_F in H3. destruct H3.
-      eapply alloc_to_FElem_F in H5; destruct H5.
-      eassert (((_ * _ * _ * _) * _)%sep mCombined2).
-      {
-        do 2 eexists; split; [eassumption | split; [| apply H12]].
-        do 2 eexists; split; [eassumption | split; [| apply H9]].
-        do 2 eexists; split; [eassumption | split; [| apply H5]].
-        do 2 eexists; split; [eassumption | split; [| apply H3]].
-        apply Hnew0.
-      }
+    split; [eapply felem_size_in_bytes_mod |].
+    repeat straightline.
+    split; [eapply felem_size_in_bytes_mod |].
+    repeat straightline.
+    split; [eapply felem_size_in_bytes_mod |].
+    repeat straightline.
+    split; [eapply felem_size_in_bytes_mod |].
+    repeat straightline.
+    eexists; split; [solve_locals5 l3 l2 l1 l0 l| ].
+
+    eapply alloc_to_FElem in H9. destruct H9.
+    eapply alloc_to_FElem in H12. destruct H12.
+    eapply Fp2_FElem_to_Fp_sep in H9, H12.
+    eapply alloc_to_FElem_F in H3. destruct H3.
+    eapply alloc_to_FElem_F in H5; destruct H5.
+    eassert (((_ * _ * _ * _) * _)%sep mCombined2).
+    {
+      do 2 eexists; split; [eassumption | split; [| apply H12]].
+      do 2 eexists; split; [eassumption | split; [| apply H9]].
+      do 2 eexists; split; [eassumption | split; [| apply H5]].
+      do 2 eexists; split; [eassumption | split; [| apply H3]].
+      apply Hnew0.
+    }
 
 
 
-      clear dependent mStack.
-      clear dependent mStack0.
-      clear dependent mStack1.
-      clear dependent mStack2.
+    clear dependent mStack.
+    clear dependent mStack0.
+    clear dependent mStack1.
+    clear dependent mStack2.
 
-      (*unfolding as multiple preconditions*)
-      (* cbv [id] in *.
+    (*unfolding as multiple preconditions*)
+    (* cbv [id] in *.
       eapply sep_and_l_fwd in H9; destruct H9 as [H9 ?].
       eapply sep_and_l_fwd in H9; destruct H9 as [H9 ?]. *)
 
-      remember (Field.FElem _ a x4) as R1.
-      remember (Field.FElem _ a0 x5) as R2.
-      remember (Field.FElem _ a1 (fst_felem x2)) as R3.
-      remember (Field.FElem _ (word.add a1 felem_offset_word) (snd_felem x2)) as R4.
-      remember (Field.FElem _ a2 (fst_felem x3)) as R5.
-      remember (Field.FElem _ (word.add a2 felem_offset_word) (snd_felem x3)) as R6.
-      eassert (( _ * (R1 * R2 * R3 * R4 * R5 * R6))%sep mCombined2) by ecancel_assumption.
-      subst R1 R2 R3 R4 R5 R6.
+    remember (Field.FElem _ a x4) as R1.
+    remember (Field.FElem _ a0 x5) as R2.
+    remember (Field.FElem _ a1 (fst_felem x2)) as R3.
+    remember (Field.FElem _ (word.add a1 felem_offset_word) (snd_felem x2)) as R4.
+    remember (Field.FElem _ a2 (fst_felem x3)) as R5.
+    remember (Field.FElem _ (word.add a2 felem_offset_word) (snd_felem x3)) as R6.
+    eassert (( _ * (R1 * R2 * R3 * R4 * R5 * R6))%sep mCombined2) by ecancel_assumption.
+    subst R1 R2 R3 R4 R5 R6.
 
-      straightline_call.
-      1: {
-        split; try ecancel_assumption.
+    straightline_call.
+    1: {
+      split; try ecancel_assumption.
 
-        eapply sep_and_l_fwd in H3; destruct H3 as [H3 ?].
-        eapply sep_and_l_fwd in H3; destruct H3 as [H3 ?].
-        ecancel_assumption.
-      }
-      repeat straightline. eapply sep_comm in H8. eapply (sep_assoc _ _ (Field.FElem _ a1 _)) in H8.
-      
-      eexists; split; [solve_locals5 l3 l2 l1 l0 l| ].
+      eapply sep_and_l_fwd in H3; destruct H3 as [H3 ?].
+      eapply sep_and_l_fwd in H3; destruct H3 as [H3 ?].
+      ecancel_assumption.
+    }
+    repeat straightline. eapply sep_comm in H8. eapply (sep_assoc _ _ (Field.FElem _ a1 _)) in H8.
 
-      straightline_call.
-      1: {
-        split; try ecancel_assumption.
-        eapply sep_and_l_fwd in H8; destruct H8 as [H8 ?].
-        eapply sep_and_l_fwd in H8; destruct H8 as [H8 ?].
-        ecancel_assumption.
-      }
-      repeat straightline. eapply sep_comm in H9. eapply (sep_assoc _ _ (Field.FElem _ (word.add a1 _) _)) in H9.
-      eexists; split; [solve_locals5 l3 l2 l1 l0 l| ].
+    eexists; split; [solve_locals5 l3 l2 l1 l0 l| ].
 
-      straightline_call.
-      1: {
-        split; try ecancel_assumption.
+    straightline_call.
+    1: {
+      split; try ecancel_assumption.
+      eapply sep_and_l_fwd in H8; destruct H8 as [H8 ?].
+      eapply sep_and_l_fwd in H8; destruct H8 as [H8 ?].
+      ecancel_assumption.
+    }
+    repeat straightline. eapply sep_comm in H9. eapply (sep_assoc _ _ (Field.FElem _ (word.add a1 _) _)) in H9.
+    eexists; split; [solve_locals5 l3 l2 l1 l0 l| ].
 
-        eapply sep_and_l_fwd in H9; destruct H9 as [H9 ?].
-        eapply sep_and_l_fwd in H9; destruct H9 as [H9 ?].
-        ecancel_assumption.
-      }
-      repeat straightline. eapply sep_comm in H11. eapply (sep_assoc _ _ (Field.FElem _ a2 _)) in H11.
-      eexists; split; [solve_locals5 l3 l2 l1 l0 l| ].
+    straightline_call.
+    1: {
+      split; try ecancel_assumption.
 
-      straightline_call.
-      1: {
-        split; try ecancel_assumption.
-        eapply sep_and_l_fwd in H11; destruct H11 as [H11 ?].
-        eapply sep_and_l_fwd in H11; destruct H11 as [H11 ?].
-        ecancel_assumption.
-      }
-      repeat straightline. eapply sep_comm in H12. eapply (sep_assoc _ _ (Field.FElem _ (word.add a2 _) _)) in H12.
-      eexists; split; [solve_locals5 l3 l2 l1 l0 l |].
+      eapply sep_and_l_fwd in H9; destruct H9 as [H9 ?].
+      eapply sep_and_l_fwd in H9; destruct H9 as [H9 ?].
+      ecancel_assumption.
+    }
+    repeat straightline. eapply sep_comm in H11. eapply (sep_assoc _ _ (Field.FElem _ a2 _)) in H11.
+    eexists; split; [solve_locals5 l3 l2 l1 l0 l| ].
 
-      (*deconstructing sep hyp.*)
-      cbv [id] in *.
-      eapply sep_and_l_fwd in H12; destruct H12 as [H12 ?].
-      eapply sep_and_l_fwd in H12; destruct H12 as [H12 ?].
-      clear H12 H5.
+    straightline_call.
+    1: {
+      split; try ecancel_assumption.
+      eapply sep_and_l_fwd in H11; destruct H11 as [H11 ?].
+      eapply sep_and_l_fwd in H11; destruct H11 as [H11 ?].
+      ecancel_assumption.
+    }
+    repeat straightline. eapply sep_comm in H12. eapply (sep_assoc _ _ (Field.FElem _ (word.add a2 _) _)) in H12.
+    eexists; split; [solve_locals5 l3 l2 l1 l0 l |].
 
-      Ltac handle_call' := straightline_call; [
-        split; [|split; [| split; [| split; [| ecancel_assumption]]]]; [| | eexists; ecancel_assumption| eexists; ecancel_assumption]; eauto
-      |].
+    (*deconstructing sep hyp.*)
+    cbv [id] in *.
+    eapply sep_and_l_fwd in H12; destruct H12 as [H12 ?].
+    eapply sep_and_l_fwd in H12; destruct H12 as [H12 ?].
+    clear H12 H5.
 
-      destruct H0, H2.
+    Ltac handle_call' := straightline_call; [
+          split; [|split; [| split; [| split; [| ecancel_assumption]]]]; [| | eexists; ecancel_assumption| eexists; ecancel_assumption]; eauto
+    |].
 
-      handle_call'.
-      repeat straightline.
-      eexists; split; [solve_locals5 l3 l2 l1 l0 l| ].
+    destruct H0, H2.
 
-      handle_call'.
-      repeat straightline.
-      eexists; split; [solve_locals5 l3 l2 l1 l0 l| ].
+    handle_call'.
+    repeat straightline.
+    eexists; split; [solve_locals5 l3 l2 l1 l0 l| ].
 
-      handle_call'.
-      repeat straightline.
-      eexists; split; [solve_locals5 l3 l2 l1 l0 l| ].
+    handle_call'.
+    repeat straightline.
+    eexists; split; [solve_locals5 l3 l2 l1 l0 l| ].
 
-      handle_call'.
-      repeat straightline.
-      eexists; split; [solve_locals5 l3 l2 l1 l0 l| ].
+    handle_call'.
+    repeat straightline.
+    eexists; split; [solve_locals5 l3 l2 l1 l0 l| ].
 
-      handle_call'.
-      repeat straightline.
-      eexists; split; [solve_locals5 l3 l2 l1 l0 l| ].
+    handle_call'.
+    repeat straightline.
+    eexists; split; [solve_locals5 l3 l2 l1 l0 l| ].
 
-      handle_call'.
-      repeat straightline.
-      eexists; split; [solve_locals5 l3 l2 l1 l0 l| ].
+    handle_call'.
+    repeat straightline.
+    eexists; split; [solve_locals5 l3 l2 l1 l0 l| ].
 
-      handle_call'.
-      repeat straightline.
-      eexists; split; [solve_locals5 l3 l2 l1 l0 l| ].
+    handle_call'.
+    repeat straightline.
+    eexists; split; [solve_locals5 l3 l2 l1 l0 l| ].
 
-      handle_call'.
-      repeat straightline.
+    handle_call'.
+    repeat straightline.
+    eexists; split; [solve_locals5 l3 l2 l1 l0 l| ].
 
-      let Hstack := (fresh "Hstack") in
-      let Hsplit := (fresh "Hsplit") in
-      let Hnew := (fresh "Hnew") in
-      eassert (Hstack : (Field.FElem _ a2 _ * _)%sep a16) by (eapply Fp_FElem_to_Fp2_R_sep; ecancel_assumption);
-      destruct Hstack as [? [? [Hsplit [Hstack' Hnew]]]]; do 2 eexists; split; [eapply FElem_Fp2_to_anybytes; eauto| split; [eapply map.split_comm; eauto| ]].
+    handle_call'.
+    repeat straightline.
 
-      let Hstack := (fresh "Hstack") in
-      let Htemp := (fresh "Htemp") in
-      let Hsplit := (fresh "Hsplit") in
-      let Hnew := (fresh "Hnew") in
-      eassert (Htemp : (Field.FElem _ a1 _ * _)%sep x15) by (eapply Fp_FElem_to_Fp2_R_sep; ecancel_assumption);
-      destruct Htemp as [? [? [Hsplit [Hstack Hnew]]]]; do 2 eexists; split; [eapply FElem_Fp2_to_anybytes; eauto| split; [eapply map.split_comm; eauto| ]].
+    let Hstack := (fresh "Hstack") in
+    let Hsplit := (fresh "Hsplit") in
+    let Hnew := (fresh "Hnew") in
+    eassert (Hstack : (Field.FElem _ a2 _ * _)%sep a16) by (eapply Fp_FElem_to_Fp2_R_sep; ecancel_assumption);
+    destruct Hstack as [? [? [Hsplit [Hstack' Hnew]]]]; do 2 eexists; split; [eapply FElem_Fp2_to_anybytes; eauto| split; [eapply map.split_comm; eauto| ]].
+
+    let Hstack := (fresh "Hstack") in
+    let Htemp := (fresh "Htemp") in
+    let Hsplit := (fresh "Hsplit") in
+    let Hnew := (fresh "Hnew") in
+    eassert (Htemp : (Field.FElem _ a1 _ * _)%sep x15) by (eapply Fp_FElem_to_Fp2_R_sep; ecancel_assumption);
+    destruct Htemp as [? [? [Hsplit [Hstack Hnew]]]]; do 2 eexists; split; [eapply FElem_Fp2_to_anybytes; eauto| split; [eapply map.split_comm; eauto| ]].
 
 
-      let Hstack := (fresh "Hstack") in
-      let Htemp := (fresh "Htemp") in
-      let Hsplit := (fresh "Hsplit") in
-      let Hnew := (fresh "Hnew") in
-      eassert (Htemp : ((Field.FElem F) a0 _ * _)%sep x17) by (ecancel_assumption);
-      destruct Htemp as [? [? [Hsplit [Hstack Hnew]]]]; do 2 eexists; split; [eapply FElem_F_to_anybytes; eauto| split; [eapply map.split_comm; eauto| ]].
+    let Hstack := (fresh "Hstack") in
+    let Htemp := (fresh "Htemp") in
+    let Hsplit := (fresh "Hsplit") in
+    let Hnew := (fresh "Hnew") in
+    eassert (Htemp : ((Field.FElem F) a0 _ * _)%sep x17) by (ecancel_assumption);
+    destruct Htemp as [? [? [Hsplit [Hstack Hnew]]]]; do 2 eexists; split; [eapply FElem_F_to_anybytes; eauto| split; [eapply map.split_comm; eauto| ]].
 
-      let Hstack := (fresh "Hstack") in
-      let Htemp := (fresh "Htemp") in
-      let Hsplit := (fresh "Hsplit") in
-      let Hnew := (fresh "Hnew") in
-      eassert (Htemp : ((Field.FElem F) a _ * _)%sep x19) by (ecancel_assumption);
-      destruct Htemp as [? [? [Hsplit [Hstack Hnew]]]]; do 2 eexists; split; [eapply FElem_F_to_anybytes; eauto| split; [eapply map.split_comm; eauto| ]].
+    let Hstack := (fresh "Hstack") in
+    let Htemp := (fresh "Htemp") in
+    let Hsplit := (fresh "Hsplit") in
+    let Hnew := (fresh "Hnew") in
+    eassert (Htemp : ((Field.FElem F) a _ * _)%sep x19) by (ecancel_assumption);
+    destruct Htemp as [? [? [Hsplit [Hstack Hnew]]]]; do 2 eexists; split; [eapply FElem_F_to_anybytes; eauto| split; [eapply map.split_comm; eauto| ]].
 
-      repeat straightline. split; auto; split; auto.
-      exists (x13 ++ x12); split; [| split].
-      1: {
-        simpl. erewrite fst_felem_app; try ecancel_assumption. erewrite snd_felem_app; try ecancel_assumption.
-        eapply Prod.path_pair.
-          - simpl.
-            (* assert (forall x, @feval *)
-            (* (@QuadraticFieldExtensionsSpecs.F_parameters prime_field_parameters) *)
-            (* width BW word mem F_representation x *)
-            (*   = (@feval F_parameters width BW word mem F_representation x)) by auto. *)
-              (* rewrite H13. *)
-              rewrite H40.
-              rewrite H16. rewrite H22.
-              eassert (Quad_non_res M_pos = _).
-              {
-                cbv [Quad_non_res]. assert (Z.pos M_pos mod 4 =? 3 = true) by lia.
-                rewrite H13.
-                eauto.
-              }
-              rewrite H13.
-              simpl.
-              Local Infix "*p" := ModularArithmetic.F.mul (at level 90).
-              Local Infix "-p" := ModularArithmetic.F.sub (at level 90).
-              Local Infix "+p" := ModularArithmetic.F.add (at level 90).
-              remember (feval (fst_felem x)) as xr.
-              remember (feval (snd_felem x)) as xi.
-              remember (feval (fst_felem y)) as yr.
-              remember (feval (snd_felem y)) as yi.
-              rewrite F_mul_assoc; [| apply M_pos_prime]. (*admitted primality of M_pos*)
-              rewrite <- H13.
-              rewrite <- mul_neg_1; eauto. apply M_pos_prime.
-          - simpl.
-            (* assert (forall x, @feval *)
-            (*   (@QuadraticFieldExtensionsSpecs.F_parameters prime_field_parameters) *)
-            (*   width BW word mem F_representation x *)
-            (*     = (@feval F_parameters width BW word mem F_representation x)) by auto. *)
-            (*   rewrite H13. *)
-              rewrite H37, H34, H31, H28, H25, H22, H16. simpl.
-              remember (feval (fst_felem x)) as xr.
-              remember (feval (snd_felem x)) as xi.
-              remember (feval (fst_felem y)) as yr.
-              remember (feval (snd_felem y)) as yi.
-              rewrite mul_equiv; eauto. apply M_pos_prime.
-      }
-      1: {
-        split.
-          - erewrite fst_felem_app; try ecancel_assumption. auto.
-          - erewrite snd_felem_app; try ecancel_assumption; auto.
-      }
-       eapply Fp_FElem_to_Fp2_R_sep. erewrite fst_felem_app; try ecancel_assumption.
-       erewrite snd_felem_app; try ecancel_assumption.
-    Qed.
-              
+    repeat straightline. split; auto; split; auto.
+    exists (x13 ++ x12); split; [| split].
+    1: {
+      simpl. erewrite fst_felem_app; try ecancel_assumption. erewrite snd_felem_app; try ecancel_assumption.
+      eapply Prod.path_pair.
+      - simpl.
+        (* assert (forall x, @feval *)
+        (* (@QuadraticFieldExtensionsSpecs.F_parameters prime_field_parameters) *)
+        (* width BW word mem F_representation x *)
+        (*   = (@feval F_parameters width BW word mem F_representation x)) by auto. *)
+        (* rewrite H13. *)
+        rewrite H40.
+        rewrite H16. rewrite H22.
+        eassert (Quad_non_res M_pos = _).
+        {
+          cbv [Quad_non_res]. assert (Z.pos M_pos mod 4 =? 3 = true) by lia.
+          rewrite H13.
+          eauto.
+        }
+        rewrite H13.
+        simpl.
+        Local Infix "*p" := ModularArithmetic.F.mul (at level 90).
+        Local Infix "-p" := ModularArithmetic.F.sub (at level 90).
+        Local Infix "+p" := ModularArithmetic.F.add (at level 90).
+        remember (feval (fst_felem x)) as xr.
+        remember (feval (snd_felem x)) as xi.
+        remember (feval (fst_felem y)) as yr.
+        remember (feval (snd_felem y)) as yi.
+        rewrite F_mul_assoc; [| apply M_pos_prime]. (*admitted primality of M_pos*)
+        rewrite <- H13.
+        rewrite <- mul_neg_1; eauto. apply M_pos_prime.
+      - simpl.
+        (* assert (forall x, @feval *)
+        (*   (@QuadraticFieldExtensionsSpecs.F_parameters prime_field_parameters) *)
+        (*   width BW word mem F_representation x *)
+        (*     = (@feval F_parameters width BW word mem F_representation x)) by auto. *)
+        (*   rewrite H13. *)
+        rewrite H37, H34, H31, H28, H25, H22, H16. simpl.
+        remember (feval (fst_felem x)) as xr.
+        remember (feval (snd_felem x)) as xi.
+        remember (feval (fst_felem y)) as yr.
+        remember (feval (snd_felem y)) as yi.
+        rewrite mul_equiv; eauto. apply M_pos_prime.
+    }
+    1: {
+      split.
+      - erewrite fst_felem_app; try ecancel_assumption. auto.
+      - erewrite snd_felem_app; try ecancel_assumption; auto.
+    }
+    eapply Fp_FElem_to_Fp2_R_sep. erewrite fst_felem_app; try ecancel_assumption.
+    erewrite snd_felem_app; try ecancel_assumption.
+  Qed.
 
-    (*subtraction in Fp2*)
-    Definition Fp2_sub : bedrock2.Syntax.func :=
-      (@Field.sub Fp2_names, (["out"; "inx"; "iny"], []:list String.string, bedrock_func_body:(
+
+  (*subtraction in Fp2*)
+  Definition Fp2_sub : bedrock2.Syntax.func :=
+    (sub (F:=Fp2), (["out"; "inx"; "iny"], []:list String.string, bedrock_func_body:(
         stackalloc (felem_size_in_bytes Fp2) as allocx;
         stackalloc (felem_size_in_bytes Fp2) as allocy;
-        coq:(cmd.call [] (fst F_copy) [expr.var ("allocx"); expr.var ("inx")]);
-        coq:(cmd.call [] (fst F_copy) [expr_2nd_felem (expr.var ("allocx")); expr_2nd_felem (expr.var ("inx"))]);
-        coq:(cmd.call [] (fst F_copy) [expr.var ("allocy"); expr.var ("iny")]);
-        coq:(cmd.call [] (fst F_copy) [expr_2nd_felem (expr.var ("allocy")); expr_2nd_felem (expr.var ("iny"))]);
-        coq:(cmd.call [] ((fst F_sub)) [expr.var "out"; expr.var "allocx"; expr.var "allocy"]);
-        coq:(cmd.call [] ((fst F_sub)) [expr_2nd_felem (expr.var "out"); expr_2nd_felem (expr.var "allocx"); expr_2nd_felem (expr.var "allocy")])
-      ))).
+        coq:(cmd.call [] (felem_copy (F:=F)) [expr.var ("allocx"); expr.var ("inx")]);
+        coq:(cmd.call [] (felem_copy (F:=F)) [expr_2nd_felem (expr.var ("allocx")); expr_2nd_felem (expr.var ("inx"))]);
+        coq:(cmd.call [] (felem_copy (F:=F)) [expr.var ("allocy"); expr.var ("iny")]);
+        coq:(cmd.call [] (felem_copy (F:=F)) [expr_2nd_felem (expr.var ("allocy")); expr_2nd_felem (expr.var ("iny"))]);
+        coq:(cmd.call [] (sub (F:=F)) [expr.var "out"; expr.var "allocx"; expr.var "allocy"]);
+        coq:(cmd.call [] (sub (F:=F)) [expr_2nd_felem (expr.var "out"); expr_2nd_felem (expr.var "allocx"); expr_2nd_felem (expr.var "allocy")])
+    ))).
   
-    Instance spec_of_Fp2_sub : spec_of (@Field.sub Fp2_names).
-    Proof.
-      simpl.
-      pose proof (@binop_spec width BW word mem locals ext_spec _ Fp2_parameters Fp2_representation (@Field.sub Fp2_names) bin_sub). cbv [spec_of]. eapply X.
-    Defined.
+  Instance spec_of_Fp2_sub : spec_of (sub (F:=Fp2)) := binop_spec bin_sub (F:=Fp2).
 
-    
-    Lemma Fp2_sub_ok : program_logic_goal_for_function! Fp2_sub.
-    Proof.
-      enter' Fp2_sub. clear H0 H1 H2 H4. cbv [binop_spec] in *.
-      intros. unfold1_call_goal. cbv match beta delta [call_body].
-      assert ((Field.sub =? Field.sub)%string = true) by (rewrite eqb_refl; auto).
-      rewrite H1.
-      cbv match beta delta [func].
-      repeat straightline.
+  Lemma Fp2_sub_ok : program_logic_goal_for_function! Fp2_sub.
+  Proof.
+    enter' Fp2_sub. clear H0 H1 H2 H4. cbv [binop_spec] in *.
+    intros. unfold1_call_goal. cbv match beta delta [call_body].
+    assert ((Field.sub =? Field.sub)%string = true) by (rewrite eqb_refl; auto).
+    rewrite H1.
+    cbv match beta delta [func].
+    repeat straightline.
 
-      eapply Fp2_FElem_to_Fp_R_sep in H4, H5, H6.
+    eapply Fp2_FElem_to_Fp_R_sep in H4, H5, H6.
 
-      collect H4 H5.
-      collect Hnew H6.
+    collect H4 H5.
+    collect Hnew H6.
 
-      split; [eapply felem_size_in_bytes_mod |].
-      repeat straightline.
-      split; [eapply felem_size_in_bytes_mod |].
-      repeat straightline.
+    split; [eapply felem_size_in_bytes_mod |].
+    repeat straightline.
+    split; [eapply felem_size_in_bytes_mod |].
+    repeat straightline.
 
-      eexists; split; [solve_locals l1 l0 l| ].
-      
-      eapply alloc_to_FElem in H4. destruct H4.
-      eapply alloc_to_FElem in H6. destruct H6.
-      eapply Fp2_FElem_to_Fp_sep in H4, H6.
-      eassert (((_ * _) * _)%sep mCombined0).
-      {
-        do 2 eexists; split; [eassumption | split; [| apply H6]].
-        do 2 eexists; split; [eassumption | split; [| apply H4]].
-        apply Hnew0.
-      }
+    eexists; split; [solve_locals l1 l0 l| ].
 
-      clear dependent mStack.
-      clear dependent mStack0.
+    eapply alloc_to_FElem in H4. destruct H4.
+    eapply alloc_to_FElem in H6. destruct H6.
+    eapply Fp2_FElem_to_Fp_sep in H4, H6.
+    eassert (((_ * _) * _)%sep mCombined0).
+    {
+      do 2 eexists; split; [eassumption | split; [| apply H6]].
+      do 2 eexists; split; [eassumption | split; [| apply H4]].
+      apply Hnew0.
+    }
 
-      (*unfolding as multiple preconditions*)
-      (* cbv [id] in *.
+    clear dependent mStack.
+    clear dependent mStack0.
+
+    (*unfolding as multiple preconditions*)
+    (* cbv [id] in *.
       eapply sep_and_l_fwd in H9; destruct H9 as [H9 ?].
       eapply sep_and_l_fwd in H9; destruct H9 as [H9 ?]. *)
 
-      remember (Field.FElem _ a (fst_felem x2)) as R1.
-      remember (Field.FElem _ a0 (fst_felem x3)) as R2.
-      remember (Field.FElem _ (word.add a felem_offset_word) (snd_felem x2)) as R3.
-      remember (Field.FElem _ (word.add a0 felem_offset_word) (snd_felem x3)) as R4.
-      eassert (( _ * (R1 * R2 * R3 * R4))%sep mCombined0) by ecancel_assumption.
-      subst R1 R2 R3 R4. clear H8.
+    remember (Field.FElem _ a (fst_felem x2)) as R1.
+    remember (Field.FElem _ a0 (fst_felem x3)) as R2.
+    remember (Field.FElem _ (word.add a felem_offset_word) (snd_felem x2)) as R3.
+    remember (Field.FElem _ (word.add a0 felem_offset_word) (snd_felem x3)) as R4.
+    eassert (( _ * (R1 * R2 * R3 * R4))%sep mCombined0) by ecancel_assumption.
+    subst R1 R2 R3 R4. clear H8.
 
-      straightline_call.
-      1: {
-        split; try ecancel_assumption.
+    straightline_call.
+    1: {
+      split; try ecancel_assumption.
 
-        eapply sep_and_l_fwd in H4; destruct H4 as [H4 ?].
-        eapply sep_and_l_fwd in H4; destruct H4 as [H4 ?].
-        ecancel_assumption.
-      }
-      repeat straightline. eapply sep_comm in H7. eapply (sep_assoc _ _ (Field.FElem _ a _)) in H7.
-      
-      eexists; split; [solve_locals l1 l0 l| ].
+      eapply sep_and_l_fwd in H4; destruct H4 as [H4 ?].
+      eapply sep_and_l_fwd in H4; destruct H4 as [H4 ?].
+      ecancel_assumption.
+    }
+    repeat straightline. eapply sep_comm in H7. eapply (sep_assoc _ _ (Field.FElem _ a _)) in H7.
 
-      straightline_call.
-      1: {
-        split; try ecancel_assumption.
-        eapply sep_and_l_fwd in H7; destruct H7 as [H7 ?].
-        eapply sep_and_l_fwd in H7; destruct H7 as [H7 ?].
-        ecancel_assumption.
-      }
-      repeat straightline. eapply sep_comm in H8. eapply (sep_assoc _ _ (Field.FElem _ (word.add a _) _)) in H8.
-      eexists; split; [solve_locals l1 l0 l| ].
+    eexists; split; [solve_locals l1 l0 l| ].
 
-      straightline_call.
-      1: {
-        split; try ecancel_assumption.
+    straightline_call.
+    1: {
+      split; try ecancel_assumption.
+      eapply sep_and_l_fwd in H7; destruct H7 as [H7 ?].
+      eapply sep_and_l_fwd in H7; destruct H7 as [H7 ?].
+      ecancel_assumption.
+    }
+    repeat straightline. eapply sep_comm in H8. eapply (sep_assoc _ _ (Field.FElem _ (word.add a _) _)) in H8.
+    eexists; split; [solve_locals l1 l0 l| ].
 
-        eapply sep_and_l_fwd in H8; destruct H8 as [H8 ?].
-        eapply sep_and_l_fwd in H8; destruct H8 as [H8 ?].
-        ecancel_assumption.
-      }
-      repeat straightline. eapply sep_comm in H9. eapply (sep_assoc _ _ (Field.FElem _ a0 _)) in H9.
-      eexists; split; [solve_locals l1 l0 l| ].
+    straightline_call.
+    1: {
+      split; try ecancel_assumption.
 
-      straightline_call.
-      1: {
-        split; try ecancel_assumption.
-        eapply sep_and_l_fwd in H9; destruct H9 as [H9 ?].
-        eapply sep_and_l_fwd in H9; destruct H9 as [H9 ?].
-        ecancel_assumption.
-      }
-      repeat straightline. eapply sep_comm in H10. eapply (sep_assoc _ _ (Field.FElem _ (word.add a0 _) _)) in H10.
-      eexists; split; [solve_locals l1 l0 l |].
+      eapply sep_and_l_fwd in H8; destruct H8 as [H8 ?].
+      eapply sep_and_l_fwd in H8; destruct H8 as [H8 ?].
+      ecancel_assumption.
+    }
+    repeat straightline. eapply sep_comm in H9. eapply (sep_assoc _ _ (Field.FElem _ a0 _)) in H9.
+    eexists; split; [solve_locals l1 l0 l| ].
 
-      (*deconstructing sep hyp.*)
-      cbv [id] in *.
-      eapply sep_and_l_fwd in H10; destruct H10 as [H10 ?].
-      eapply sep_and_l_fwd in H10; destruct H10 as [H10 ?].
-      clear H10 H6.
+    straightline_call.
+    1: {
+      split; try ecancel_assumption.
+      eapply sep_and_l_fwd in H9; destruct H9 as [H9 ?].
+      eapply sep_and_l_fwd in H9; destruct H9 as [H9 ?].
+      ecancel_assumption.
+    }
+    repeat straightline. eapply sep_comm in H10. eapply (sep_assoc _ _ (Field.FElem _ (word.add a0 _) _)) in H10.
+    eexists; split; [solve_locals l1 l0 l |].
+
+    (*deconstructing sep hyp.*)
+    cbv [id] in *.
+    eapply sep_and_l_fwd in H10; destruct H10 as [H10 ?].
+    eapply sep_and_l_fwd in H10; destruct H10 as [H10 ?].
+    clear H10 H6.
 
 
-      destruct H0, H2.
+    destruct H0, H2.
 
-      handle_call'.
-      repeat straightline.
-      eexists; split; [solve_locals l1 l0 l| ].
+    handle_call'.
+    repeat straightline.
+    eexists; split; [solve_locals l1 l0 l| ].
 
-      handle_call'.
-      repeat straightline.
+    handle_call'.
+    repeat straightline.
 
-      let Hstack := (fresh "Hstack") in
-      let Hsplit := (fresh "Hsplit") in
-      let Hnew := (fresh "Hnew") in
-      eassert (Hstack : (Field.FElem _ a0 _ * _)%sep a8) by (eapply Fp_FElem_to_Fp2_R_sep; ecancel_assumption);
-      destruct Hstack as [? [? [Hsplit [Hstack' Hnew]]]]; do 2 eexists; split; [eapply FElem_Fp2_to_anybytes; eauto| split; [eapply map.split_comm; eauto| ]].
+    let Hstack := (fresh "Hstack") in
+    let Hsplit := (fresh "Hsplit") in
+    let Hnew := (fresh "Hnew") in
+    eassert (Hstack : (Field.FElem _ a0 _ * _)%sep a8) by (eapply Fp_FElem_to_Fp2_R_sep; ecancel_assumption);
+    destruct Hstack as [? [? [Hsplit [Hstack' Hnew]]]]; do 2 eexists; split; [eapply FElem_Fp2_to_anybytes; eauto| split; [eapply map.split_comm; eauto| ]].
 
-      let Hstack := (fresh "Hstack") in
-      let Htemp := (fresh "Htemp") in
-      let Hsplit := (fresh "Hsplit") in
-      let Hnew := (fresh "Hnew") in
-      eassert (Htemp : (Field.FElem _ a _ * _)%sep x7) by (eapply Fp_FElem_to_Fp2_R_sep; ecancel_assumption);
-      destruct Htemp as [? [? [Hsplit [Hstack Hnew]]]]; do 2 eexists; split; [eapply FElem_Fp2_to_anybytes; eauto| split; [eapply map.split_comm; eauto| ]].
+    let Hstack := (fresh "Hstack") in
+    let Htemp := (fresh "Htemp") in
+    let Hsplit := (fresh "Hsplit") in
+    let Hnew := (fresh "Hnew") in
+    eassert (Htemp : (Field.FElem _ a _ * _)%sep x7) by (eapply Fp_FElem_to_Fp2_R_sep; ecancel_assumption);
+    destruct Htemp as [? [? [Hsplit [Hstack Hnew]]]]; do 2 eexists; split; [eapply FElem_Fp2_to_anybytes; eauto| split; [eapply map.split_comm; eauto| ]].
 
-      repeat straightline. split; auto; split; auto.
-      exists (x4 ++ x5); split; [| split].
-      1: {
-        simpl. erewrite fst_felem_app; try ecancel_assumption. erewrite snd_felem_app; try ecancel_assumption.
-        eapply Prod.path_pair; auto.
-      }
-      1: {
-        split.
-          - erewrite fst_felem_app; try ecancel_assumption; auto.
-          - erewrite snd_felem_app; try ecancel_assumption; auto.
-      }
-       eapply Fp_FElem_to_Fp2_R_sep. erewrite fst_felem_app; try ecancel_assumption.
-       erewrite snd_felem_app; try ecancel_assumption.
-    Qed.
+    repeat straightline. split; auto; split; auto.
+    exists (x4 ++ x5); split; [| split].
+    1: {
+      simpl. erewrite fst_felem_app; try ecancel_assumption. erewrite snd_felem_app; try ecancel_assumption.
+      eapply Prod.path_pair; auto.
+    }
+    1: {
+      split.
+      - erewrite fst_felem_app; try ecancel_assumption; auto.
+      - erewrite snd_felem_app; try ecancel_assumption; auto.
+    }
+    eapply Fp_FElem_to_Fp2_R_sep. erewrite fst_felem_app; try ecancel_assumption.
+    erewrite snd_felem_app; try ecancel_assumption.
+  Qed.
 
 End Fp2.
