src/Bedrock/Field/Synthesis/Examples/bls12_Fp2.v
@@ -1,33 +1,48 @@
-Require Import Crypto.Bedrock.Specs.Field.
-Require Import Crypto.Bedrock.Field.Synthesis.New.WordByWordMontgomery.
-Require Import Crypto.Bedrock.Field.Synthesis.Examples.bls12_prime.
-Require Import Crypto.Bedrock.Field.Synthesis.Examples.felem_copy_p224.
-Require Import Crypto.Bedrock.Field.FieldExtensions.QuadraticFieldExtensions.
 Require Import Coq.Strings.String.
-Local Open Scope string_scope. Local Open Scope Z_scope. Local Open Scope list_scope.
-
 Require Import bedrock2.NotationsCustomEntry.
 Require Import bedrock2.WeakestPrecondition.
 Require Import Crypto.Bedrock.Field.FieldExtensions.QuadraticFieldExtensionsSpecs.
 Require Import Rupicola.Lib.Api.
 Require Import Crypto.Bedrock.Field.Interface.Compilation2.
+Require Import Crypto.Bedrock.Specs.Field.
+Require Import Crypto.Bedrock.Field.Synthesis.New.WordByWordMontgomery.
+Require Import Crypto.Bedrock.Field.Synthesis.Examples.bls12_prime.
+Require Import Crypto.Bedrock.Field.Synthesis.Examples.felem_copy_p224.
+Require Import Crypto.Bedrock.Field.FieldExtensions.QuadraticFieldExtensions.
 
-Import Syntax BinInt String List.ListNotations.
+Import BinInt String List.ListNotations.
+
+Local Open Scope string_scope.
+Local Open Scope Z_scope.
+Local Open Scope list_scope.
 
 Section bls12_Fp2.
 
-    Existing Instances Defaults64.default_parameters Defaults64.default_parameters_ok.
+    Existing Instances
+      Defaults64.default_parameters
+      Defaults64.default_parameters_ok
+      bls12_prime_parameters
+      (* bls12_field_parameters *)
+      bls12_field_names
+      bls12_field_representation.
 
-    Existing Instance prime_parameters.
+    Local Notation Fp2 := ((F M_pos) * (F M_pos))%type.
+
+    Instance bls12_Fp2_field_parameters : FieldParameters Fp2 := Fp2_field_parameters.
+    Instance bls12_Fp2_field_representation : FieldRepresentation Fp2 := Fp2_field_representation.
+
+    Instance spec_of_bls12_add : spec_of add := spec_of_F_add.
+    Instance spec_of_bls12_mul : spec_of mul := spec_of_F_mul.
+    Instance spec_of_bls12_sub : spec_of sub := spec_of_F_sub.
+    Instance spec_of_bls12_felem_copy : spec_of felem_copy := spec_of_F_felem_copy.
+    Instance spec_of_bls12_select_znz : spec_of select_znz := spec_of_F_select_znz.
+
     Let prefix := "bls12_Fp2".
+    Instance bls12_Fp2_field_names : FieldNames Fp2 := field_names_prefixed Fp2 prefix.
 
-    Instance F_names : FieldNames := field_names.
-    Instance Fp2_names : FieldNames := field_names_prefixed prefix.
-    (* Check Fp2_representation. *)
-
-    Definition bls12_Fp2_add := (@Fp2_add _ _ _ _ bls12_prime.prime_parameters F_names (field_representation ) (snd bls12_add) (snd felem_copy_func) Fp2_names).
-    Definition bls12_Fp2_mul := (@Fp2_mul _ _ _ _ bls12_prime.prime_parameters F_names (field_representation ) (snd bls12_add) (snd felem_copy_func) (snd bls12_sub) (snd bls12_mul) Fp2_names).
-    Definition bls12_Fp2_sub := (@Fp2_sub _ _ _ _ bls12_prime.prime_parameters F_names (field_representation ) (snd bls12_sub) (snd felem_copy_func) Fp2_names).
+    Instance spec_of_bls12_Fp2_add : spec_of (add (F:=Fp2)) := spec_of_Fp2_add.
+    Instance spec_of_bls12_Fp2_mul : spec_of (mul (F:=Fp2)) := spec_of_Fp2_mul.
+    Instance spec_of_bls12_Fp2_sub : spec_of (sub (F:=Fp2)) := spec_of_Fp2_sub.
 
     (*Print rest of functions to C*)
     (* From bedrock2 Require Import ToCString Bytedump.
@@ -36,55 +51,20 @@ Section bls12_Fp2.
 
     Eval compute in c_mod. *)
 
-    Instance spec_of_bls12_add : spec_of (fst bls12_add).
-    Proof.
-        exact (@spec_of_add _ _ _ _ _ _ bls12_prime.prime_parameters F_names (field_representation)).
-    Defined.
-
-    Instance spec_of_bls12_Fp2_add : spec_of (fst bls12_Fp2_add).
-    Proof.
-        exact (@spec_of_Fp2_add _ _ _ _ _ _ bls12_prime.prime_parameters (field_representation) Fp2_names).
-    Defined.
-
-    Instance spec_of_bls12_mul : spec_of (fst bls12_mul).
-    Proof.
-        exact (@spec_of_F_mul _ _ _ _ _ _ bls12_prime.prime_parameters F_names (field_representation )).
-    Defined.
-
-    Instance spec_of_bls12_Fp2_mul : spec_of (fst bls12_Fp2_mul).
-    Proof.
-        exact (@spec_of_Fp2_mul _ _ _ _ _ _ bls12_prime.prime_parameters (field_representation ) Fp2_names).
-    Defined.
-
-    Instance spec_of_bls12_sub : spec_of (fst bls12_sub).
-    Proof.
-        exact (@spec_of_F_sub _ _ _ _ _ _ bls12_prime.prime_parameters F_names (field_representation )).
-    Defined.
-
-    Instance spec_of_bls12_Fp2_sub : spec_of (fst bls12_Fp2_sub).
-    Proof.
-        exact (@spec_of_Fp2_sub _ _ _ _ _ _ bls12_prime.prime_parameters (field_representation ) Fp2_names).
-    Defined.
-
-    Instance spec_of_bls12_felem_copy : spec_of ((@felem_copy F_names)).
-    Proof.
-        exact spec_of_felem_copy. (* (@Field.spec_of_felem_copy _ _ _ _ _ _ (F M_pos) field_parameters F_names (field_representation )). *)
-    Defined.
-
-    Lemma bls12_Fp2_add_ok : program_logic_goal_for_function! bls12_Fp2_add.
+    Lemma bls12_Fp2_add_ok : program_logic_goal_for_function! Fp2_add.
     Proof.
         eapply Fp2_add_ok.
         Unshelve. all: try eapply Defaults64.default_parameters_ok; auto.
     Qed.
 
-    Lemma bls12_Fp2_sub_ok : program_logic_goal_for_function! bls12_Fp2_sub.
+    Lemma bls12_Fp2_sub_ok : program_logic_goal_for_function! Fp2_sub.
     Proof.
         eapply Fp2_sub_ok.
         (* epose proof (Fp2_sub_ok). cbv [bls12_Fp2_sub]. eapply (H (snd felem_copy_func) (snd bls12_sub)). *)
         Unshelve. all: try eapply Defaults64.default_parameters_ok; auto.
     Qed.
 
-    Lemma bls12_Fp2_mul_ok : program_logic_goal_for_function! bls12_Fp2_mul.
+    Lemma bls12_Fp2_mul_ok : program_logic_goal_for_function! Fp2_mul.
     Proof.
         eapply Fp2_mul_ok.
         (* epose proof (Fp2_mul_ok). eapply H. *)
