src/Bedrock/Field/Synthesis/Examples/bls12_prime.v
@@ -28,75 +28,71 @@ Section Field.
   Definition n : nat := 6.
   Definition u := -0xd201000000010000.
   Definition p_of_u u := (((u - 1)^2 * (u^4 - u^2 + 1)) / 3) + u.
-  Definition m := Eval compute in (p_of_u u).
+  (* Definition m := Eval compute in (p_of_u u). *)
 
-  Eval compute in m.
+  Existing Instances
+    Defaults64.default_parameters
+    Defaults64.default_parameters_ok
+    no_select_size
+    split_mul_to
+    split_multiret_to.
 
-  Existing Instances Defaults64.default_parameters
-           Defaults64.default_parameters_ok.
-  Existing Instances no_select_size split_mul_to split_multiret_to.
   Definition prefix : string := "bls12_"%string.
 
-  Instance prime_parameters : PrimeParameters.
+  Instance bls12_prime_parameters : PrimeParameters.
   Proof using Type.
-    let M := (eval vm_compute in (Z.to_pos (m))) in
+    let M := (eval vm_compute in (Z.to_pos (p_of_u u))) in
     exact (Build_PrimeParameters M).
-    (* (* curve 'A' parameter *) *)
-    (* let a := constr:(F.of_Z M (m - 3)) in *)
-    (* let prefix := constr:("bls12_"%string) in *)
-    (* eapply *)
-    (*   (field_parameters_prefixed *)
-    (*      M ((a - F.of_Z _ 2) / F.of_Z _ 4)%F prefix). *)
   Defined.
 
-  Local Notation F := (F (Z.to_pos m)).
+  Local Notation F := (F M_pos).
 
-  Instance field_names : FieldNames := field_names_prefixed prefix.
-  Instance field_parameters : FieldParameters F := prime_field_parameters.
-  (* Existing Instance prime_field_parameters. *)
+  Instance bls12_field_names : FieldNames F := field_names_prefixed F prefix.
+  Instance bls12_field_parameters : FieldParameters F := prime_field_parameters.
+  Instance bls12_field_representation : FieldRepresentation F := field_representation.
 
   Definition to_mont_string := prefix ++ "to_mont".
   Definition from_mont_string := prefix ++ "from_mont".
 
   (* Call fiat-crypto pipeline on all field operations *)
-Instance bls12_ops : @word_by_word_Montgomery_ops from_mont_string to_mont_string _ _ _ _ _ _ _ _ _ _ _ _ (WordByWordMontgomery.n m machine_wordsize) m.
-Proof using Type. Time constructor; make_computed_op. Defined.
+  Instance bls12_ops : @word_by_word_Montgomery_ops from_mont_string to_mont_string _ _ _ _ _ _ _ _ _ _ _ _ (WordByWordMontgomery.n M machine_wordsize) M.
+  Proof using Type. Time constructor; make_computed_op. Defined.
 
   (**** Translate each field operation into bedrock2 and apply bedrock2 backend
         field pipeline proofs to prove the bedrock2 functions are correct. ****)
 
-        Local Ltac begin_derive_bedrock2_func :=
-        lazymatch goal with
-        | |- context [spec_of_BinOp bin_mul] => eapply mul_func_correct
-        | |- context [spec_of_UnOp un_square] => eapply square_func_correct
-        | |- context [spec_of_BinOp bin_add] => eapply add_func_correct
-        | |- context [spec_of_BinOp bin_sub] => eapply sub_func_correct
-        | |- context [spec_of_UnOp un_opp] => eapply opp_func_correct
-        (* | |- context [spec_of_UnOp un_scmula24] => eapply scmula24_func_correct *)
-        | |- context [spec_of_from_bytes] => eapply from_bytes_func_correct
-        | |- context [spec_of_to_bytes] => eapply to_bytes_func_correct
-        end.
-      
-      Ltac derive_bedrock2_func op :=
-        begin_derive_bedrock2_func;
-        (* this goal fills in the evar, so do it first for [abstract] to be happy *)
-        try lazymatch goal with
-            | |- _ = b2_func _ => vm_compute; reflexivity
-            end;
-        (* solve all the remaining goals *)
-        lazymatch goal with
-        | |- _ = @ErrorT.Success ?ErrT unit tt =>
-          abstract (vm_cast_no_check (@eq_refl _ (@ErrorT.Success ErrT unit tt)))
-        | |- Func.valid_func _ =>
-          eapply Func.valid_func_bool_iff;
-          abstract vm_cast_no_check (eq_refl true)
-        | |- (_ = _)%Z => vm_compute; reflexivity
-        end.
+  Local Ltac begin_derive_bedrock2_func :=
+    lazymatch goal with
+    | |- context [spec_of_BinOp bin_mul] => eapply mul_func_correct
+    | |- context [spec_of_UnOp un_square] => eapply square_func_correct
+    | |- context [spec_of_BinOp bin_add] => eapply add_func_correct
+    | |- context [spec_of_BinOp bin_sub] => eapply sub_func_correct
+    | |- context [spec_of_UnOp un_opp] => eapply opp_func_correct
+    (* | |- context [spec_of_UnOp un_scmula24] => eapply scmula24_func_correct *)
+    | |- context [spec_of_from_bytes] => eapply from_bytes_func_correct
+    | |- context [spec_of_to_bytes] => eapply to_bytes_func_correct
+    end.
+
+  Ltac derive_bedrock2_func op :=
+    begin_derive_bedrock2_func;
+    (* this goal fills in the evar, so do it first for [abstract] to be happy *)
+    try lazymatch goal with
+      | |- _ = b2_func _ => vm_compute; reflexivity
+      end;
+    (* solve all the remaining goals *)
+    lazymatch goal with
+    | |- _ = @ErrorT.Success ?ErrT unit tt =>
+      abstract (vm_cast_no_check (@eq_refl _ (@ErrorT.Success ErrT unit tt)))
+    | |- Func.valid_func _ =>
+      eapply Func.valid_func_bool_iff;
+      abstract vm_cast_no_check (eq_refl true)
+    | |- (_ = _)%Z => vm_compute; reflexivity
+    end.
 
   Derive bls12_from_bytes
          SuchThat (forall functions,
                       spec_of_from_bytes
-                        (field_representation:=field_representation_raw m)
+                        (field_representation:=field_representation_raw)
                         (bls12_from_bytes :: functions))
          As bls12_from_bytes_correct.
   Proof. Time derive_bedrock2_func from_bytes_op. Qed.
@@ -104,7 +100,7 @@ Proof using Type. Time constructor; make_computed_op. Defined.
   Derive bls12_to_bytes
          SuchThat (forall functions,
                       spec_of_to_bytes
-                        (field_representation:=field_representation_raw m)
+                        (field_representation:=field_representation_raw)
                         (bls12_to_bytes :: functions))
          As bls12_to_bytes_correct.
   Proof. Time derive_bedrock2_func to_bytes_op. Qed.
@@ -112,7 +108,7 @@ Proof using Type. Time constructor; make_computed_op. Defined.
   Derive bls12_mul
          SuchThat (forall functions,
                       spec_of_BinOp bin_mul
-                        (field_representation:=field_representation m)
+                        (field_representation:=field_representation)
                         (bls12_mul :: functions))
          As bls12_mul_correct.
   Proof. Time derive_bedrock2_func mul_op. Qed.
@@ -120,7 +116,7 @@ Proof using Type. Time constructor; make_computed_op. Defined.
   Derive bls12_square
          SuchThat (forall functions,
                       spec_of_UnOp un_square
-                        (field_representation:=field_representation m)
+                        (field_representation:=field_representation)
                         (bls12_square :: functions))
          As bls12_square_correct.
   Proof. Time derive_bedrock2_func square_op. Qed.
@@ -128,7 +124,7 @@ Proof using Type. Time constructor; make_computed_op. Defined.
   Derive bls12_add
          SuchThat (forall functions,
                       spec_of_BinOp bin_add
-                        (field_representation:=field_representation m)
+                        (field_representation:=field_representation)
                         (bls12_add :: functions))
          As bls12_add_correct.
   Proof. Time derive_bedrock2_func add_op. Qed.
@@ -136,7 +132,7 @@ Proof using Type. Time constructor; make_computed_op. Defined.
   Derive bls12_sub
          SuchThat (forall functions,
                       spec_of_BinOp bin_sub
-                        (field_representation:=field_representation m)
+                        (field_representation:=field_representation)
                         (bls12_sub :: functions))
          As bls12_sub_correct.
   Proof. Time derive_bedrock2_func sub_op. Qed.
@@ -145,26 +141,25 @@ Proof using Type. Time constructor; make_computed_op. Defined.
   Derive bls12_from_mont
          SuchThat (forall functions,
                       spec_of_UnOp un_from_mont
-                        (field_representation:=field_representation m)
+                        (field_representation:=field_representation)
                         (bls12_from_mont :: functions))
          As bls12_from_mont_correct.
   Proof.
-    eapply (from_mont_func_correct _ _ _ from_mont_string to_mont_string); auto.
+    eapply (from_mont_func_correct _ from_mont_string to_mont_string); auto.
         - vm_compute; reflexivity.
         - eapply Func.valid_func_bool_iff. abstract vm_cast_no_check (eq_refl true).
           Unshelve.
-            + auto.
             + auto.
   Qed.
 
   Derive bls12_to_mont
          SuchThat (forall functions,
                       spec_of_UnOp un_to_mont
-                        (field_representation:=field_representation m)
+                        (field_representation:=field_representation)
                         (bls12_to_mont :: functions))
          As to_from_mont_correct.
   Proof.
-    eapply (to_mont_func_correct _ _ _ from_mont_string to_mont_string); auto.
+    eapply (to_mont_func_correct _ from_mont_string to_mont_string); auto.
         - vm_compute; reflexivity.
         - eapply Func.valid_func_bool_iff. abstract vm_cast_no_check (eq_refl true).
           Unshelve. all: auto.
@@ -173,7 +168,7 @@ Proof using Type. Time constructor; make_computed_op. Defined.
   Derive bls12_select_znz
            SuchThat (forall functions,
                       spec_of_selectznz
-                        (field_representation:=field_representation m)
+                        (field_representation:=field_representation)
                         (bls12_select_znz :: functions))
          As select_znz_correct.
   Proof.
@@ -190,9 +185,6 @@ Proof using Type. Time constructor; make_computed_op. Defined.
        [ bls12_select_znz].
      
      Compute compile (compile_ext_call (funname_env:=SortedListString.map)) (map.of_list funcs).
-
-
-
 
      From bedrock2 Require Import ToCString Bytedump.
      Check c_module.
